CIU implies CTX

src/FrameStack/CTX.v
@@ -19,7 +19,7 @@ Definition CompatibleFun (R : nat -> Exp -> Exp -> Prop) :=
     R Γ (EFun vl e1) (EFun vl' e2).
 
 Definition CompatibleValues (R : nat -> Exp -> Exp -> Prop) :=
-  forall Γ el el', length el = length el' ->
+  forall Γ el el',
     Forall (fun e => EXP Γ ⊢ e) el ->
     Forall (fun e => EXP Γ ⊢ e) el' ->
     list_biforall (R Γ) el el' ->
@@ -34,35 +34,38 @@ Definition CompatibleCons (R : nat -> Exp -> Exp -> Prop) :=
     R Γ (ECons e1 e2) (ECons e1' e2').
 
 Definition CompatibleTuple (R : nat -> Exp -> Exp -> Prop) :=
-  forall Γ el el', length el = length el' ->
+  forall Γ el el',
     Forall (fun e => EXP Γ ⊢ e) el ->
     Forall (fun e => EXP Γ ⊢ e) el' ->
     list_biforall (R Γ) el el' ->
     R Γ (ETuple el) (ETuple el').
 
 Definition CompatibleMap (R : nat -> Exp -> Exp -> Prop) :=
-  forall Γ l l', length l = length l' ->
+  forall Γ l l',
     Forall (PBoth (fun e => EXP Γ ⊢ e)) l ->
     Forall (PBoth (fun e => EXP Γ ⊢ e)) l' ->
     list_biforall (fun '(v1, v2) '(v1', v2') => R Γ v1 v1' /\ R Γ v2 v2') l l' ->
     R Γ (EMap l) (EMap l').
 
 Definition CompatibleCall (R : nat -> Exp -> Exp -> Prop) :=
-  forall Γ m m' f f' el el', m = m' -> f = f' -> length el = length el' ->
+  forall Γ m m' f f' el el',
+  EXP Γ ⊢ m -> EXP Γ ⊢ m' ->
+  EXP Γ ⊢ f -> EXP Γ ⊢ f' ->
+  R Γ m m' -> R Γ f f' ->
   Forall (fun e => EXP Γ ⊢ e) el ->
   Forall (fun e => EXP Γ ⊢ e) el' ->
   list_biforall (R Γ) el el' ->
     R Γ (ECall m f el) (ECall m' f' el').
 
 Definition CompatiblePrimOp (R : nat -> Exp -> Exp -> Prop) :=
-  forall Γ f f' el el', f = f' -> length el = length el' ->
+  forall Γ f f' el el', f = f' ->
     Forall (fun e => EXP Γ ⊢ e) el ->
     Forall (fun e => EXP Γ ⊢ e) el' ->
     list_biforall (R Γ) el el' ->
     R Γ (EPrimOp f el) (EPrimOp f' el').
 
 Definition CompatibleApp (R : nat -> Exp -> Exp -> Prop) :=
-  forall Γ e e' el el', length el = length el' ->
+  forall Γ e e' el el',
     EXP Γ ⊢ e ->
     EXP Γ ⊢ e' ->
     Forall (fun e => EXP Γ ⊢ e) el ->
@@ -72,7 +75,7 @@ Definition CompatibleApp (R : nat -> Exp -> Exp -> Prop) :=
     R Γ (EApp e el) (EApp e' el').
 
 Definition CompatibleCase (R : nat -> Exp -> Exp -> Prop) := (* TODO: l or l' in places? *)
-  forall Γ e e' l l', length l = length l' ->
+  forall Γ e e' l l',
     EXP Γ ⊢ e ->
     EXP Γ ⊢ e' ->
     Forall (fun '(p, g, e) => EXP PatListScope p + Γ ⊢ g /\ EXP PatListScope p + Γ ⊢ e) l ->
@@ -106,7 +109,7 @@ Definition CompatibleSeq (R : nat -> Exp -> Exp -> Prop) :=
     R Γ (ESeq e1 e2) (ESeq e1' e2').
 
 Definition CompatibleLetRec (R : nat -> Exp -> Exp -> Prop) :=
-  forall Γ e l e' l', length l = length l' ->
+  forall Γ e l e' l',
     EXP (length l  + Γ) ⊢ e  ->
     EXP (length l' + Γ) ⊢ e' ->
     Forall (fun '(vl, e) => EXP length l + vl + Γ ⊢ e) l  ->
@@ -311,7 +314,8 @@ Proof.
     auto.
   * unfold CompatibleLetRec.
     intros.
-    auto.
+    apply Erel_LetRec_compat; auto.
+    now apply biforall_length in H3.
   * unfold CompatibleTry.
     intros.
     auto.
@@ -338,40 +342,41 @@ Proof.
     apply CIU_iff_Rrel, Rrel_exp_compat_reverse in H2. now apply Erel_IsPreCtxRel.
   * intros ?; intros.
     apply CIU_iff_Rrel. apply Rrel_exp_compat.
-    eapply biforall_impl in H2. 2: { intros; apply CIU_iff_Rrel, Rrel_exp_compat_reverse in H3. exact H3. }
+    eapply biforall_impl in H1. 2: { intros; apply CIU_iff_Rrel, Rrel_exp_compat_reverse in H2. exact H2. }
     now apply Erel_IsPreCtxRel.
   * intros ?; intros.
     apply CIU_iff_Rrel. apply Rrel_exp_compat.
     apply CIU_iff_Rrel, Rrel_exp_compat_reverse in H3, H4. now apply Erel_IsPreCtxRel.
   * intros ?; intros.
     apply CIU_iff_Rrel. apply Rrel_exp_compat.
+    eapply biforall_impl in H1. 2: { intros; apply CIU_iff_Rrel, Rrel_exp_compat_reverse in H2. exact H2. }
+    now apply Erel_IsPreCtxRel.
+  * intros ?; intros.
+    apply CIU_iff_Rrel. apply Rrel_exp_compat.
+    apply biforall_impl with (Q := fun '(v1, v2) '(v1', v2') => Erel_open Γ v1 v1' /\ Erel_open Γ v2 v2') in H1. 2: { intros. destruct x, y, H2.
+    apply CIU_iff_Rrel, Rrel_exp_compat_reverse in H2, H3.
+    pose proof (conj H2 H3). exact H4. }
+    now apply Erel_IsPreCtxRel.
+  * intros ?; intros.
+    apply CIU_iff_Rrel, Rrel_exp_compat_reverse in H3, H4.
+    apply CIU_iff_Rrel. apply Rrel_exp_compat.
+    eapply biforall_impl in H7. 2: { intros. apply CIU_iff_Rrel, Rrel_exp_compat_reverse in H8. exact H8. }
+    now apply Erel_IsPreCtxRel.
+  * intros ?; intros.
+    apply CIU_iff_Rrel. apply Rrel_exp_compat.
     eapply biforall_impl in H2. 2: { intros; apply CIU_iff_Rrel, Rrel_exp_compat_reverse in H3. exact H3. }
     now apply Erel_IsPreCtxRel.
   * intros ?; intros.
     apply CIU_iff_Rrel. apply Rrel_exp_compat.
-    apply biforall_impl with (Q := fun '(v1, v2) '(v1', v2') => Erel_open Γ v1 v1' /\ Erel_open Γ v2 v2') in H2. 2: { intros. destruct x, y, H3.
-    apply CIU_iff_Rrel, Rrel_exp_compat_reverse in H3, H4.
-    pose proof (conj H3 H4). exact H5. }
-    now apply Erel_IsPreCtxRel.
-  * intros ?; intros.
-    apply CIU_iff_Rrel. apply Rrel_exp_compat.
+    apply CIU_iff_Rrel, Rrel_exp_compat_reverse in H3.
     eapply biforall_impl in H4. 2: { intros; apply CIU_iff_Rrel, Rrel_exp_compat_reverse in H5. exact H5. }
     now apply Erel_IsPreCtxRel.
   * intros ?; intros.
     apply CIU_iff_Rrel. apply Rrel_exp_compat.
-    eapply biforall_impl in H3. 2: { intros; apply CIU_iff_Rrel, Rrel_exp_compat_reverse in H4. exact H4. }
-    now apply Erel_IsPreCtxRel.
-  * intros ?; intros.
-    apply CIU_iff_Rrel. apply Rrel_exp_compat.
-    apply CIU_iff_Rrel, Rrel_exp_compat_reverse in H4.
-    eapply biforall_impl in H5. 2: { intros; apply CIU_iff_Rrel, Rrel_exp_compat_reverse in H6. exact H6. }
-    now apply Erel_IsPreCtxRel.
-  * intros ?; intros.
-    apply CIU_iff_Rrel. apply Rrel_exp_compat.
-    apply CIU_iff_Rrel, Rrel_exp_compat_reverse in H4.
+    apply CIU_iff_Rrel, Rrel_exp_compat_reverse in H3.
     apply biforall_impl with (Q := fun '(p, g, e) '(p', g', e') =>
-        p = p' /\ Erel_open (PatListScope p + Γ) g g' /\ Erel_open (PatListScope p + Γ) e e') in H5. 2: { intros. destruct x, p, y, p, H6, H7.
-    apply CIU_iff_Rrel, Rrel_exp_compat_reverse in H7, H8.
+        p = p' /\ Erel_open (PatListScope p + Γ) g g' /\ Erel_open (PatListScope p + Γ) e e') in H4. 2: { intros. destruct x, p, y, p, H5, H6.
+    apply CIU_iff_Rrel, Rrel_exp_compat_reverse in H6, H7.
     intuition. }
     now apply Erel_IsPreCtxRel.
   * intros ?; intros.
@@ -382,15 +387,1006 @@ Proof.
     apply CIU_iff_Rrel, Rrel_exp_compat_reverse in H3, H4. now apply Erel_IsPreCtxRel.
   * intros ?; intros.
     apply CIU_iff_Rrel. apply Rrel_exp_compat.
-    apply CIU_iff_Rrel, Rrel_exp_compat_reverse in H5.
-    apply biforall_impl with (Q := fun '(v, e) '(v', e') => v = v' /\ Erel_open (Datatypes.length l + v + Γ) e e') in H4. 2: { intros. destruct x, y, H6.
-    apply CIU_iff_Rrel, Rrel_exp_compat_reverse in H7. intuition. }
+    apply CIU_iff_Rrel, Rrel_exp_compat_reverse in H4.
+    apply biforall_impl with (Q := fun '(v, e) '(v', e') => v = v' /\ Erel_open (Datatypes.length l + v + Γ) e e') in H3. 2: { intros. destruct x, y, H5.
+    apply CIU_iff_Rrel, Rrel_exp_compat_reverse in H6. intuition. }
     now apply Erel_IsPreCtxRel.
   * intros ?; intros.
     apply CIU_iff_Rrel. apply Rrel_exp_compat.
     apply CIU_iff_Rrel, Rrel_exp_compat_reverse in H7, H8, H9.
     now apply Erel_IsPreCtxRel.
 Qed.
+
+Inductive CtxIdent :=
+| CValues
+| CTuple
+| CMap
+| CCall (e1 e2 : Exp)
+| CPrimOp (f : string)
+| CApp (e : Exp).
+
+Inductive Ctx :=
+| CHole
+| CFun     (vl : nat) (c : Ctx)
+| CParams  (ident : CtxIdent) (el : list Exp) (c : Ctx) (el' : list Exp)
+| CCons1   (c : Ctx) (tl : Exp)
+| CCons2   (hd : Exp) (c : Ctx)
+| CCallMod (c : Ctx) (f : Exp) (l : list Exp)
+| CCallFun (m : Exp) (c : Ctx) (l : list Exp)
+| CApp1    (c : Ctx) (l : list Exp)
+| CCase1   (c : Ctx) (l : list ((list Pat) * Exp * Exp))
+| CCase2   (e : Exp) (l : list ((list Pat) * Exp * Exp)) (lp : (list Pat)) (c : Ctx) (e2 : Exp) (l' : list ((list Pat) * Exp * Exp))
+| CCase3   (e : Exp) (l : list ((list Pat) * Exp * Exp)) (lp : (list Pat)) (e1 : Exp) (c : Ctx) (l' : list ((list Pat) * Exp * Exp))
+| CLet1    (l : nat) (c : Ctx) (e2 : Exp)
+| CLet2    (l : nat) (e1: Exp) (c : Ctx)
+| CSeq1    (c : Ctx) (e2 : Exp)
+| CSeq2    (e1 : Exp) (c : Ctx)
+| CLetRec1 (l : list (nat * Exp)) (n : nat) (c : Ctx) (l' : list (nat * Exp)) (e : Exp)
+| CLetRec2 (l : list (nat * Exp)) (c : Ctx)
+| CTry1    (c : Ctx) (vl1 : nat) (e2 : Exp) (vl2 : nat) (e3 : Exp)
+| CTry2    (e1 : Exp) (vl1 : nat) (c : Ctx) (vl2 : nat) (e3 : Exp)
+| CTry3    (e1 : Exp) (vl1 : nat) (e2 : Exp) (vl2 : nat) (c : Ctx)
+.
+
+Definition create_exp (ident : CtxIdent) (l : list Exp) :=
+match ident with
+ | CValues => EValues l
+ | CTuple => ETuple l
+ | CMap => EMap (deflatten_list l)
+ | CCall e1 e2 => ECall e1 e2 l
+ | CPrimOp f => EPrimOp f l
+ | CApp e => EApp e l
+end.
+
+
+Fixpoint plug (C : Ctx) (p : Exp) :=
+match C with
+| CHole              => p
+| CFun    vl c       => EExp ( EFun vl (plug c p) )
+| CCons1  c tl       => EExp ( ECons (plug c p) tl )
+| CCons2  hd c       => EExp ( ECons hd (plug c p) )
+| CParams ident l c l'
+                     => EExp ( create_exp ident (l ++ [(plug c p)] ++ l') )
+| CCallMod c f l     => EExp ( ECall (plug c p) f l )
+| CCallFun m c l     => EExp ( ECall m (plug c p) l )
+| CApp1   c l        => EExp ( EApp (plug c p) l )
+| CCase1  c l        => EExp ( ECase (plug c p) l )
+| CCase2  e l lp c e2 l' => EExp ( ECase e (l ++ [(lp, (plug c p), e2)] ++ l') )
+| CCase3  e l lp e1 c l' => EExp ( ECase e (l ++ [(lp, e1, (plug c p))] ++ l') )
+| CLet1   l c e2     => EExp ( ELet l (plug c p) e2 )
+| CLet2   l e1 c     => EExp ( ELet l e1 (plug c p) )
+| CSeq1   c e2       => EExp ( ESeq (plug c p) e2 )
+| CSeq2   e1 c       => EExp ( ESeq e1 (plug c p) )
+| CLetRec1 l n c l' e => EExp ( ELetRec (l ++ [(n, (plug c p))] ++ l') e )
+| CLetRec2 l c     => EExp ( ELetRec l (plug c p) )
+| CTry1   c vl1 e2 vl2 e3  => EExp ( ETry (plug c p) vl1 e2 vl2 e3 )
+| CTry2   e1 vl1 c vl2 e3  => EExp ( ETry e1 vl1 (plug c p) vl2 e3 )
+| CTry3   e1 vl1 e2 vl2 c  => EExp ( ETry e1 vl1 e2 vl2 (plug c p) )
+end.
+
+Fixpoint plugc (C : Ctx) (p : Ctx) :=
+match C with
+| CHole             => p
+| CFun    vl c      => CFun vl (plugc c p)
+| CCons1  c tl      => CCons1 (plugc c p) tl
+| CCons2  hd c      => CCons2 hd (plugc c p)
+| CParams ident l c l' => CParams ident l (plugc c p) l'
+| CCallMod c f l    => CCallMod (plugc c p) f l
+| CCallFun m c l    => CCallFun m (plugc c p) l
+| CApp1   c l       => CApp1 (plugc c p) l
+| CCase1  c l       => CCase1 (plugc c p) l
+| CCase2  e l lp c e2 l' => CCase2 e l lp (plugc c p) e2 l'
+| CCase3  e l lp e1 c l' => CCase3 e l lp e1 (plugc c p) l'
+| CLet1   l c e2    => CLet1 l (plugc c p) e2
+| CLet2   l e1 c    => CLet2 l e1 (plugc c p)
+| CSeq1   c e2      => CSeq1 (plugc c p) e2
+| CSeq2   e1 c      => CSeq2 e1 (plugc c p)
+| CLetRec1 l n c l' e => CLetRec1 l n (plugc c p) l' e
+| CLetRec2 l c      => CLetRec2 l (plugc c p)
+| CTry1   c vl1 e2 vl2 e3  => CTry1 (plugc c p) vl1 e2 vl2 e3
+| CTry2   e1 vl1 c vl2 e3  => CTry2 e1 vl1 (plugc c p) vl2 e3
+| CTry3   e1 vl1 e2 vl2 c  => CTry3 e1 vl1 e2 vl2 (plugc c p)
+end.
+
+
+Lemma plug_assoc : forall C1 C2 e,
+    plug C1 (plug C2 e) =
+    plug (plugc C1 C2) e.
+Proof.
+  induction C1;
+    intros;
+    cbn;
+    auto;
+    try rewrite IHC1;
+    auto.
+Qed.
+
+Reserved Notation "'EECTX' Γh ⊢ C ∷ Γ" (at level 60).
+Reserved Notation "'EECTXID' Γh ⊢ C ∷ Γ" (at level 60).
+(* Reserved Notation "'VECTX' Γh ⊢ C ∷ Γ" (at level 60). *)
+
+Inductive EECtxIdentScope (Γh : nat) : CtxIdent -> nat -> Prop :=
+
+| CEScope_CValues Γ : EECTXID Γh ⊢ CValues ∷ Γ
+
+| CEScope_CTuple Γ : EECTXID Γh ⊢ CTuple ∷ Γ
+
+| CEScope_CMap Γ : EECTXID Γh ⊢ CMap ∷ Γ
+
+| CEScope_CPrimOp Γ f : EECTXID Γh ⊢ CPrimOp f ∷ Γ
+
+| CEScope_CCall Γ m f : EXP Γ ⊢ m -> EXP Γ ⊢ f ->
+                        EECTXID Γh ⊢ CCall m f ∷ Γ
+
+| CEScope_CApp Γ e : EXP Γ ⊢ e -> EECTXID Γh ⊢ CApp e ∷ Γ
+
+where "'EECTXID' Γh ⊢ C ∷ Γ" := (EECtxIdentScope Γh C Γ).
+
+Inductive EECtxScope (Γh : nat) : nat -> Ctx -> Prop :=
+
+| CEScope_Hole : (EECTX Γh ⊢ CHole ∷ Γh)
+
+| CEScope_CFun : forall Γ vl c,
+  EECTX Γh ⊢ c ∷ (vl + Γ) -> 
+  EECTX Γh ⊢ (CFun vl c) ∷ Γ
+
+| CEScope_CCons1 : forall Γ c tl,
+  EECTX Γh ⊢ c ∷ Γ ->
+  EXP Γ ⊢ tl ->
+  EECTX Γh ⊢ (CCons1 c tl) ∷ Γ
+
+| CEScope_CCons2 : forall Γ hd c,
+  EXP Γ ⊢ hd ->
+  EECTX Γh ⊢ c ∷ Γ ->
+  EECTX Γh ⊢ (CCons2 hd c) ∷ Γ
+
+| CEScope_CParams : forall Γ ident l c l',
+  (ident = CMap -> exists n, length l + length l' = 1 + 2 * n) ->
+  Forall (fun e => EXP Γ ⊢ e) l ->
+  EECTX Γh ⊢ c ∷ Γ ->
+  Forall (fun e => EXP Γ ⊢ e) l' ->
+  EECTXID Γh ⊢ ident ∷ Γ ->
+  EECTX Γh ⊢ (CParams ident l c l') ∷ Γ
+
+| CEScope_CCallMod : forall Γ c f l,
+  EECTX Γh ⊢ c ∷ Γ ->
+  EXP Γ ⊢ f ->
+  Forall (fun e => EXP Γ ⊢ e) l ->
+  EECTX Γh ⊢ CCallMod c f l ∷ Γ
+
+| CEScope_CCallFun : forall Γ m c l,
+  EXP Γ ⊢ m ->
+  EECTX Γh ⊢ c ∷ Γ ->
+  Forall (fun e => EXP Γ ⊢ e) l ->
+  EECTX Γh ⊢ CCallFun m c l ∷ Γ
+
+| CEScope_CApp1 : forall Γ c l,
+  EECTX Γh ⊢ c ∷ Γ ->
+  Forall (fun e => EXP Γ ⊢ e) l ->
+  EECTX Γh ⊢ (CApp1 c l) ∷ Γ
+
+| CEScope_CCase1 : forall Γ c l,
+  EECTX Γh ⊢ c ∷ Γ ->
+  Forall (fun '(p, g, e) => EXP PatListScope p + Γ ⊢ g /\ EXP PatListScope p + Γ ⊢ e) l ->
+  EECTX Γh ⊢ (CCase1 c l) ∷ Γ
+
+
+| CEScope_CCase2 : forall Γ e l lp c e2 l',
+  EXP Γ ⊢ e ->
+  EXP PatListScope lp + Γ ⊢ e2 ->
+  Forall (fun '(p, g, e) => EXP PatListScope p + Γ ⊢ g /\ EXP PatListScope p + Γ ⊢ e) l ->
+  Forall (fun '(p, g, e) => EXP PatListScope p + Γ ⊢ g /\ EXP PatListScope p + Γ ⊢ e) l' ->
+  EECTX Γh ⊢ c ∷ ((PatListScope lp) + Γ) ->
+  EECTX Γh ⊢ (CCase2 e l lp c e2 l') ∷ Γ
+
+| CEScope_CCase3 : forall Γ e l lp e1 c l',
+  EXP Γ ⊢ e ->
+  EXP (PatListScope lp + Γ) ⊢ e1 ->
+  Forall (fun '(p, g, e) => EXP PatListScope p + Γ ⊢ g /\ EXP PatListScope p + Γ ⊢ e) l ->
+  Forall (fun '(p, g, e) => EXP PatListScope p + Γ ⊢ g /\ EXP PatListScope p + Γ ⊢ e) l' ->
+  EECTX Γh ⊢ c ∷ ((PatListScope lp) + Γ) ->
+  EECTX Γh ⊢ (CCase3 e l lp e1 c l') ∷ Γ
+
+| CEScope_CLet1 : forall Γ l c e2,
+  EECTX Γh ⊢ c ∷ Γ ->
+  EXP (l + Γ) ⊢ e2 ->
+  EECTX Γh ⊢ (CLet1 l c e2) ∷ Γ
+
+| CEScope_CLet2 : forall Γ l e1 c,
+  EXP Γ ⊢ e1 ->
+  EECTX Γh ⊢ c ∷ (l + Γ) ->
+  EECTX Γh ⊢ (CLet2 l e1 c) ∷ Γ
+
+| CEScope_CSeq1 : forall Γ c e2,
+  EECTX Γh ⊢ c ∷ Γ ->
+  EXP Γ ⊢ e2 ->
+  EECTX Γh ⊢ (CSeq1 c e2) ∷ Γ
+
+| CEScope_CSeq2 : forall Γ e1 c,
+  EXP Γ ⊢ e1 ->
+  EECTX Γh ⊢ c ∷ Γ ->
+  EECTX Γh ⊢ (CSeq2 e1 c) ∷ Γ
+
+| CEScope_CLetRec1 : forall Γ l n c l' e,
+  Forall (fun '(vl, e) => EXP length l + S (length l') + vl + Γ ⊢ e) l  ->
+  EECTX Γh ⊢ c ∷ ((length l) + S (length l') + n + Γ) ->
+  Forall (fun '(vl, e) => EXP length l + S (length l') + vl + Γ ⊢ e) l'  ->
+  EXP (length l + S (length l') + Γ) ⊢ e ->
+  EECTX Γh ⊢ (CLetRec1 l n c l' e) ∷ Γ
+
+| CEScope_CLetRec2 : forall Γ l c,
+  Forall (fun '(vl, e) => EXP length l + vl + Γ ⊢ e) l  ->
+  EECTX Γh ⊢ c ∷ (length l + Γ) ->
+  EECTX Γh ⊢ (CLetRec2 l c) ∷ Γ
+
+| CEScope_CTry1 : forall Γ c vl1 e2 vl2 e3,
+  EECTX Γh ⊢ c ∷ Γ ->
+  EXP (vl1 + Γ) ⊢ e2 ->
+  EXP (vl2 + Γ) ⊢ e3 ->
+  EECTX Γh ⊢ (CTry1 c vl1 e2 vl2 e3) ∷ Γ
+
+| CEScope_CTry2 : forall Γ e1 vl1 c vl2 e3,
+  EXP Γ ⊢ e1 ->
+  EECTX Γh ⊢ c ∷ (vl1 + Γ) ->
+  EXP (vl2 + Γ) ⊢ e3 ->
+  EECTX Γh ⊢ (CTry2 e1 vl1 c vl2 e3) ∷ Γ
+
+| CEScope_CTry3 : forall Γ e1 vl1 e2 vl2 c,
+  EXP Γ ⊢ e1 ->
+  EXP (vl1 + Γ) ⊢ e2 ->
+  EECTX Γh ⊢ c ∷ (vl2 + Γ) ->
+  EECTX Γh ⊢ (CTry3 e1 vl1 e2 vl2 c) ∷ Γ
+
+where
+"'EECTX' Γh ⊢ C ∷ Γ" := (EECtxScope Γh Γ C)
+.
+
+
+Ltac solve_inversion :=
+  match goal with
+  | [ H : _ |- _ ] => solve [inv H]
+  end.
+
+Lemma plug_preserves_scope_exp : forall {Γh C Γ e},
+    (EECTX Γh ⊢ C ∷ Γ ->
+     EXP Γh ⊢ e ->
+     EXP Γ ⊢ plug C e).
+Proof.
+  induction C; intros; inv H; subst; simpl; try (now (do 2 constructor; auto)); auto.
+  * destruct ident; inv H10; do 2 constructor; try (apply indexed_to_forall;
+    apply Forall_app; split; auto); auto.
+    all: erewrite <- map_length; apply indexed_to_forall; apply List.Forall_map.
+    all: apply Forall_impl with (P := fun '(x, y) => EXP Γ ⊢ x /\ EXP Γ ⊢ y); [destruct a; intro G; now destruct G|].
+    all: apply deflatten_keeps_prop_match.
+    all: apply Forall_app; split; auto.
+  * do 2 constructor. apply indexed_to_forall. all: auto.
+  * do 2 constructor. apply indexed_to_forall. all: auto.
+  * do 2 constructor. 2: apply indexed_to_forall. all: auto.
+  * do 2 constructor.
+    - now apply IHC.
+    - rewrite indexed_to_forall with (def := ([], `VNil, `VNil)) in H5.
+      intros. rewrite map_nth with (d := ([], `VNil, `VNil)).
+      extract_map_fun F. replace [] with (F ([], `VNil, `VNil)) at 1 by now subst F.
+      rewrite map_nth. subst F. apply H5 in H. destruct nth, p. cbn. apply H.
+    - rewrite indexed_to_forall with (def := ([], `VNil, `VNil)) in H5.
+      intros. rewrite map_nth with (d := ([], `VNil, `VNil)).
+      extract_map_fun F. replace [] with (F ([], `VNil, `VNil)) at 1 by now subst F.
+      rewrite map_nth. subst F. apply H5 in H. destruct nth, p. cbn. apply H.
+  * do 2 constructor; auto; rewrite indexed_to_forall with (def := ([], `VNil, `VNil)) in H11, H10.
+    all: intros; rewrite map_nth with (d := ([], `VNil, `VNil));
+    extract_map_fun F; replace [] with (F ([], `VNil, `VNil)) at 1 by now subst F.
+    rewrite map_nth. 2: rewrite map_nth. (* this does not wotk in `all:` somewhy... *)
+    all: subst F.
+    all: apply nth_possibilities_alt with (def := ([], `VNil, `VNil)) in H; intuition.
+    - apply H10 in H2. destruct nth, p, nth, p. inv H. cbn. apply H2.
+    - simpl in H1. rewrite app_nth2; auto. remember (i - length l) as i'.
+      destruct i'; cbn. now apply IHC.
+      specialize (H11 i' ltac:(lia)). destruct nth, p. apply H11.
+    - rewrite app_nth1; auto. specialize (H10 i ltac:(lia)). destruct nth, p. apply H10.
+    - simpl in H1. rewrite app_nth2; auto. remember (i - length l) as i'.
+      destruct i'; cbn. auto. 
+      specialize (H11 i' ltac:(lia)). destruct nth, p. apply H11.
+  * do 2 constructor; auto; rewrite indexed_to_forall with (def := ([], `VNil, `VNil)) in H11, H10.
+    all: intros; rewrite map_nth with (d := ([], `VNil, `VNil));
+    extract_map_fun F; replace [] with (F ([], `VNil, `VNil)) at 1 by now subst F.
+    rewrite map_nth. 2: rewrite map_nth. (* this does not wotk in `all:` somewhy... *)
+    all: subst F.
+    all: apply nth_possibilities_alt with (def := ([], `VNil, `VNil)) in H; intuition.
+    - apply H10 in H2. destruct nth, p, nth, p. inv H. cbn. apply H2.
+    - simpl in H1. rewrite app_nth2; auto. remember (i - length l) as i'.
+      destruct i'; cbn. auto.
+      specialize (H11 i' ltac:(lia)). destruct nth, p. apply H11.
+    - rewrite app_nth1; auto. specialize (H10 i ltac:(lia)). destruct nth, p. apply H10.
+    - simpl in H1. rewrite app_nth2; auto. remember (i - length l) as i'.
+      destruct i'; cbn. now apply IHC.
+      specialize (H11 i' ltac:(lia)). destruct nth, p. apply H11.
+  * do 2 constructor; auto; rewrite indexed_to_forall with (def := (0, `VNil)) in H6, H9.
+    2: rewrite app_length; simpl; assumption.
+    intros. do 2 rewrite map_nth with (d := (0, `VNil)).
+    apply nth_possibilities_alt with (def := (0, `VNil)) in H; intuition.
+    - rewrite app_nth1; auto. apply H6 in H2. rewrite app_length. simpl.
+      now destruct (nth i l (0, `VNil)).
+    - simpl in H1. rewrite app_nth2; auto. remember (i - length l) as i'.
+      destruct i'; cbn. rewrite app_length. now apply IHC.
+      specialize (H9 i' ltac:(lia)). rewrite app_length. destruct nth. apply H9.
+  * do 2 constructor. 2: now apply IHC.
+    intros. rewrite indexed_to_forall with (def := (0, `VNil)) in H4. apply H4 in H.
+    do 2 rewrite map_nth with (d := (0, `VNil)). now destruct nth.
+Qed.
+
+Lemma plugc_preserves_scope_exp : forall {Γh Couter Γ Cinner Γ'},
+    (EECTX Γ' ⊢ Couter ∷ Γ ->
+     EECTX Γh ⊢ Cinner ∷ Γ' ->
+     EECTX Γh ⊢ plugc Couter Cinner ∷ Γ).
+Proof.
+  induction Couter;
+    intros;
+    inv H;
+    try solve_inversion;
+    auto;
+    constructor;
+    firstorder idtac.
+  inv H10; now constructor.
+Qed.
+
+
+(* In CTX, we only care about syntax, thus only expressions can be considered as
+   equivalent. However, in CIU/LogRel, we have the possibility to do that for exceptions
+   too. This also can be expressed with CTX by ECall "erlang" "error" [reason;details] *)
+Definition CTX (Γ : nat) (e1 e2 : Exp) :=
+  (EXP Γ ⊢ e1 /\ EXP Γ ⊢ e2) /\
+  (forall (C : Ctx),
+      EECTX Γ ⊢ C ∷ 0 -> | [], RExp (plug C e1) | ↓ -> | [], RExp (plug C e2) | ↓).
+
+Lemma IsReflexiveList : forall R' l Γ',
+  IsReflexive R' -> Forall (fun r => EXP Γ' ⊢ r) l ->
+  Forall (fun '(e0, e3) => R' Γ' e0 e3) (combine l l).
+Proof.
+  induction l; intros; constructor.
+  * apply H. inversion H0. auto.
+  * inversion H0. apply IHl; auto.
+Qed.
+
+Lemma biforall_IsReflexive :
+  forall (R : nat -> Exp -> Exp -> Prop), IsReflexive R ->
+  forall l Γ, Forall (fun e : Exp => EXP Γ ⊢ e) l -> list_biforall (R Γ) l l.
+Proof.
+  induction l; constructor; auto.
+  inv H0. now apply H. inv H0. now apply IHl.
+Qed.
+
+Lemma CTX_bigger : forall R' : nat -> Exp -> Exp -> Prop,
+    IsPreCtxRel R' -> forall (Γ : nat) (e1 e2 : Exp), R' Γ e1 e2 -> CTX Γ e1 e2.
+Proof.
+  intros R' HR.
+  destruct HR as [Rscope [Radequate [Rrefl [Rtrans [RFun [ RValues [RCons [RTuple [RMap  [ RCall [ RPrimOp [RApp [RCase [RLet [RSeq [RLetRec RTry ] ] ] ] ] ] ] ] ] ] ] ] ] ] ] ].
+  unfold CTX.
+  intros.
+  destruct (Rscope _ _ _ H) as [Hscope_e1 Hscope_e2].
+  intuition idtac. eapply Radequate; eauto.
+  assert (forall Γ', EECTX Γ ⊢ C ∷ Γ' -> 
+                     R' Γ' (plug C e1) (plug C e2)).
+  { clear H0 H1.
+    induction C;
+      intros;
+      inv H0;
+      cbn;
+      try solve_inversion;
+      auto.
+    - apply RFun. reflexivity.
+      1-2: eapply plug_preserves_scope_exp; eauto.
+      apply IHC; auto.
+    - inv H10; [apply RValues | apply RTuple | apply RMap | apply RPrimOp | apply RCall | apply RApp ]; auto.
+      all: try (try apply deflatten_keeps_prop; apply Forall_app; split; auto; constructor; auto).
+      all: try (eapply plug_preserves_scope_exp; eauto).
+      3: apply deflatten_keeps_biprop_match.
+      all: apply biforall_app; [now apply biforall_IsReflexive | constructor; [|now apply biforall_IsReflexive]].
+      all: now apply IHC.
+    - apply RCons; auto.
+      + eapply @plug_preserves_scope_exp with (e := e1) in H4; eauto 2.
+      + eapply @plug_preserves_scope_exp with (e := e2) in H4; eauto 2.
+    - apply RCons; auto.
+      + eapply @plug_preserves_scope_exp with (e := e1) in H5; eauto 2.
+      + eapply @plug_preserves_scope_exp with (e := e2) in H5; eauto 2.
+    - apply RCall; auto.
+      1-2: eapply plug_preserves_scope_exp; eauto.
+      apply forall_biforall_refl, Forall_forall. intros.
+      rewrite Forall_forall in H7. now apply Rrefl, H7.
+    - apply RCall; auto.
+      1-2: eapply plug_preserves_scope_exp; eauto.
+      apply forall_biforall_refl, Forall_forall. intros.
+      rewrite Forall_forall in H7. now apply Rrefl, H7.
+    - apply RApp; auto.
+      + eapply @plug_preserves_scope_exp with (e := e1) in H4; eauto 2.
+      + eapply @plug_preserves_scope_exp with (e := e2) in H4; eauto 2.
+      + apply forall_biforall_refl.
+        apply Forall_forall. rewrite Forall_forall in H5. intros. apply Rrefl. auto.
+    - apply RCase; auto.
+      + eapply @plug_preserves_scope_exp with (e := e1) in H4; eauto 2.
+      + eapply @plug_preserves_scope_exp with (e := e2) in H4; eauto 2.
+      + apply forall_biforall_refl.
+        apply Forall_forall. rewrite Forall_forall in H5. intros.
+        destruct x, p. split. 2: split. reflexivity.
+        all: apply Rrefl; now apply H5 in H0.
+    - apply RCase; auto.
+      1-2: apply Forall_app; split; auto; constructor; auto.
+      1-2: simpl; split; try eapply plug_preserves_scope_exp; eauto.
+      apply biforall_app. 2: constructor.
+      + apply forall_biforall_refl, Forall_forall. intros.
+        rewrite Forall_forall in H10. destruct x, p. split. 2: split.
+        reflexivity.
+        all: apply Rrefl; now apply H10 in H0.
+      + split; auto.
+      + apply forall_biforall_refl, Forall_forall. intros.
+        rewrite Forall_forall in H11. destruct x, p. split. 2: split.
+        reflexivity.
+        all: apply Rrefl; now apply H11 in H0.
+    - apply RCase; auto.
+      1-2: apply Forall_app; split; auto; constructor; auto.
+      1-2: simpl; split; try eapply plug_preserves_scope_exp; eauto.
+      apply biforall_app. 2: constructor.
+      + apply forall_biforall_refl, Forall_forall. intros.
+        rewrite Forall_forall in H10. destruct x, p. split. 2: split.
+        reflexivity.
+        all: apply Rrefl; now apply H10 in H0.
+      + split; auto.
+      + apply forall_biforall_refl, Forall_forall. intros.
+        rewrite Forall_forall in H11. destruct x, p. split. 2: split.
+        reflexivity.
+        all: apply Rrefl; now apply H11 in H0.
+    - apply RLet; auto.
+      + eapply @plug_preserves_scope_exp with (e := e1) in H4; eauto 2.
+      + eapply @plug_preserves_scope_exp with (e := e2) in H4; eauto 2.
+    - apply RLet; auto.
+      + eapply @plug_preserves_scope_exp with (e := e1) in H6; eauto 2.
+      + eapply @plug_preserves_scope_exp with (e := e2) in H6; eauto 2.
+    - apply RSeq; auto.
+      + eapply @plug_preserves_scope_exp with (e := e1) in H4; eauto 2.
+      + eapply @plug_preserves_scope_exp with (e := e2) in H4; eauto 2.
+    - apply RSeq; auto.
+      + eapply @plug_preserves_scope_exp with (e := e1) in H5; eauto 2.
+      + eapply @plug_preserves_scope_exp with (e := e2) in H5; eauto 2.
+    - apply RLetRec; auto.
+      + rewrite app_length. eauto.
+      + rewrite app_length. eauto.
+      + apply Forall_app. split. rewrite app_length. exact H6.
+        constructor. eapply plug_preserves_scope_exp. rewrite app_length.
+        exact H8. auto.
+        rewrite app_length. exact H9.
+      + apply Forall_app. split. rewrite app_length. exact H6.
+        constructor. eapply plug_preserves_scope_exp. rewrite app_length.
+        exact H8. auto.
+        rewrite app_length. exact H9.
+      + rewrite app_length in *. apply biforall_app. 2: constructor.
+        ** apply forall_biforall_refl, Forall_forall. intros.
+           rewrite Forall_forall in H6. destruct x. split. reflexivity.
+           apply Rrefl; now apply H6 in H0.
+        ** split; auto.
+        ** apply forall_biforall_refl, Forall_forall. intros.
+           rewrite Forall_forall in H9. destruct x. split. reflexivity.
+           apply Rrefl; now apply H9 in H0.
+      + apply Rrefl. rewrite app_length; auto.
+    - apply RLetRec; auto.
+      + eapply @plug_preserves_scope_exp with (e := e1) in H5; eauto 2.
+      + eapply @plug_preserves_scope_exp with (e := e2) in H5; eauto 2.
+      + apply forall_biforall_refl, Forall_forall. intros.
+        rewrite Forall_forall in H4. destruct x. split. reflexivity.
+        apply Rrefl; now apply H4 in H0.
+    - apply RTry; auto.
+      + eapply @plug_preserves_scope_exp with (e := e1) in H5; eauto 2.
+      + eapply @plug_preserves_scope_exp with (e := e2) in H5; eauto 2.
+    - apply RTry; auto.
+      + eapply @plug_preserves_scope_exp with (e := e1) in H8; eauto 2.
+      + eapply @plug_preserves_scope_exp with (e := e2) in H8; eauto 2.
+    - apply RTry; auto.
+      + eapply @plug_preserves_scope_exp with (e := e1) in H9; eauto 2.
+      + eapply @plug_preserves_scope_exp with (e := e2) in H9; eauto 2.
+  }
+  now apply H2.
+Qed.
+
+Corollary CIU_implies_CTX :
+  forall Γ (e1 e2 : Exp), CIU_open Γ e1 e2 -> CTX Γ e1 e2.
+Proof.
+  intros. eapply CTX_bigger. apply CIU_IsPreCtxRel. assumption.
+Qed.
+
+
+Theorem CTX_refl Γ e : EXP Γ ⊢ e -> CTX Γ e e.
+Proof.
+  unfold CTX. intros. split; auto.
+Qed.
+
+Lemma CTX_IsPreCtxRel : IsPreCtxRel CTX.
+Proof.
+  unfold IsPreCtxRel.
+  intuition idtac;
+    try solve
+        [unfold CTX in H; intuition idtac
+        |inversion H; [|constructor]; apply H0].
+  * unfold Adequate.
+    intros.
+    unfold CTX in H.
+    intuition idtac.
+    - apply (H2 CHole); auto.
+      constructor.
+  * unfold IsReflexive.
+    intros.
+    unfold CTX.
+    intuition (auto using Rbar_le_refl).
+  * unfold Transitive.
+    intros.
+    unfold CTX in *.
+    intuition idtac.
+    auto.
+  * unfold CompatibleFun.
+    intros.
+    unfold CTX in *.
+    intuition auto.
+    specialize (H4 (plugc C (CFun vl' CHole))).
+    repeat rewrite <- plug_assoc in H4.
+    cbn in H4.
+    apply H4.
+    eapply plugc_preserves_scope_exp; eauto.
+    constructor. subst. constructor. now subst.
+  * unfold CompatibleValues.
+    intros. unfold CTX in *.
+    intuition auto.
+    1-2: do 2 constructor; rewrite <- indexed_to_forall; eassumption.
+    clear H H0. generalize dependent C. induction H1; intros.
+    - assumption.
+    - replace (plug C (° EValues (hd :: tl))) with
+              (plug (plugc C (CValues [] CHole tl)) hd) in H3 
+        by now rewrite <- plug_assoc.
+      destruct H. apply H0 in H3.
+      
+  * unfold CompatibleApp.
+    intros.
+    unfold CTX in *.
+    intuition auto.
+    1-2: rewrite indexed_to_forall in H, H0; constructor; auto.
+    clear H3 H7.
+    assert (EECTX Γ ⊢ plugc C (CAppFun CHole vals1) ∷ 0) as HC_e1.
+    { eapply plugc_preserves_scope_exp; eauto.
+      constructor; auto.
+      constructor.
+    }
+    apply H6 in HC_e1. 2: rewrite <- plug_assoc in *; simpl; auto.
+    apply biforall_length in H4 as LL. rewrite <- plug_assoc in HC_e1.
+    destruct vals1; intros.
+    - inversion H4. now subst.
+    - inversion H4. subst. destruct H9, H3. inversion H. inversion H0. subst.
+      assert (EECTX Γ ⊢ plugc C (CAppParam f2 [] CHole vals1) ∷ 0). {
+        eapply plugc_preserves_scope_exp; eauto.
+        constructor; auto.
+        constructor.
+      }
+      apply H7 in H10. 2: now rewrite <- plug_assoc.
+      replace (hd' :: tl') with ([] ++ [hd'] ++ tl') by auto.
+      eapply PreCTX_app_helper; eauto.
+      now rewrite plug_assoc.
+  * unfold CompatibleLet.
+    intros.
+    unfold CTX in *.
+    intuition auto.
+    clear H5 H9 H4 H8.
+    assert (EECTX Γ ⊢ plugc C (CLet1 x CHole e2) ∷ 0) as HC_e1.
+    { eapply plugc_preserves_scope_exp; eauto.
+      constructor; auto.
+      constructor.
+    }
+    assert (EECTX S Γ ⊢ plugc C (CLet2 x e1' CHole) ∷ 0) as HC_e2.
+    { eapply plugc_preserves_scope_exp; eauto.
+      constructor; auto.
+      constructor.
+    }
+    apply H6 in HC_e1. 2: rewrite <- plug_assoc in *; simpl; auto.
+    apply H7 in HC_e2. 2: rewrite <- plug_assoc in *; simpl; auto.
+    rewrite <- plug_assoc in HC_e2. simpl in HC_e2.
+    shelve.
+  * unfold CompatibleLetRec.
+    intros.
+    unfold CTX in *.
+    intuition auto.
+    rewrite H in H1; constructor; auto.
+    clear H5 H9 H6 H10.
+    assert (EECTX S (length vl) + Γ ⊢ plugc C (CLetRec1 f vl CHole e2) ∷ 0) as HC_e1.
+    { eapply plugc_preserves_scope_exp; eauto.
+      constructor; auto.
+      constructor.
+    }
+    assert (EECTX S Γ ⊢ plugc C (CLetRec2 f vl b1' CHole) ∷ 0) as HC_e2.
+    { eapply plugc_preserves_scope_exp; eauto.
+      constructor; auto.
+      constructor.
+    }
+    apply H7 in HC_e1. 2: rewrite <- plug_assoc in *; simpl; auto.
+    apply H8 in HC_e2. 2: rewrite <- plug_assoc in *; simpl; auto.
+    rewrite <- plug_assoc in HC_e2. simpl in HC_e2.
+    shelve.
+  * unfold CompatibleCase.
+    intros.
+    unfold CTX in *.
+    intuition auto.
+    clear H7 H12 H8 H13 H5 H14.
+    assert (EECTX Γ ⊢ plugc C (CCase1 CHole p e2 e3) ∷ 0) as HC_e1.
+    { eapply plugc_preserves_scope_exp; eauto.
+      constructor; auto.
+      constructor.
+    }
+    apply H9 in HC_e1. 2: rewrite <- plug_assoc; simpl; auto.
+    assert (EECTX pat_vars p + Γ ⊢ plugc C (CCase2 e1' p CHole e3) ∷ 0) as HC_e2.
+    { eapply plugc_preserves_scope_exp; eauto.
+      constructor; auto.
+      constructor.
+    }
+    apply H10 in HC_e2. 2: { rewrite <- plug_assoc in *; simpl in *; auto. }
+    assert (EECTX Γ ⊢ plugc C (CCase3 e1' p e2' CHole) ∷ 0) as HC_e3.
+    { eapply plugc_preserves_scope_exp; eauto.
+      constructor; auto.
+      constructor.
+    }
+    apply H11 in HC_e3. 2: { rewrite <- plug_assoc in *; simpl in *; auto. }
+    rewrite <- plug_assoc in HC_e3. simpl in HC_e3. auto.
+  * unfold CompatibleCons.
+    intros.
+    unfold CTX in *.
+    intuition auto.
+    clear H4 H8 H5 H9.
+    assert (EECTX Γ ⊢ plugc C (CCons1 e1 CHole) ∷ 0) as HC_e1.
+    { eapply plugc_preserves_scope_exp; eauto.
+      constructor; auto.
+      constructor.
+    }
+    apply H7 in HC_e1. 2: rewrite <- plug_assoc; simpl; auto.
+    assert (EECTX Γ ⊢ plugc C (CCons2 CHole e2') ∷ 0) as HC_e2.
+    { eapply plugc_preserves_scope_exp; eauto.
+      constructor; auto.
+      constructor.
+    }
+    apply H6 in HC_e2. 2: rewrite <- plug_assoc in *; simpl; auto.
+    rewrite <- plug_assoc in HC_e2. simpl in HC_e2; auto.
+  * unfold CompatibleBIF.
+    intros.
+    unfold CTX in *.
+    intuition auto.
+    1-2: rewrite indexed_to_forall in H, H0; constructor; auto.
+    clear H3 H7.
+    assert (EECTX Γ ⊢ plugc C (CBIFFun CHole vals1) ∷ 0) as HC_e1.
+    { eapply plugc_preserves_scope_exp; eauto.
+      constructor; auto.
+      constructor.
+    }
+    apply H6 in HC_e1. 2: rewrite <- plug_assoc in *; simpl; auto.
+    apply biforall_length in H4 as LL. rewrite <- plug_assoc in HC_e1.
+    destruct vals1; intros.
+    - inversion H4. now subst.
+    - inversion H4. subst. destruct H9, H3. inversion H. inversion H0. subst.
+      assert (EECTX Γ ⊢ plugc C (CBIFParam f2 [] CHole vals1) ∷ 0). {
+        eapply plugc_preserves_scope_exp; eauto.
+        constructor; auto.
+        constructor.
+      }
+      apply H7 in H10. 2: now rewrite <- plug_assoc.
+      replace (hd' :: tl') with ([] ++ [hd'] ++ tl') by auto.
+      eapply PreCTX_BIF_helper; eauto.
+      now rewrite plug_assoc.
+  * unfold CompatibleReceive.
+    intros.
+    unfold CTX in *.
+    split. split.
+    (** TODO: will be changed *)
+    3: { intros. destruct l, l2. 2-3: inversion H1.
+         auto.
+         destruct p, p0. inversion H1. subst. destruct H7 as [H7_1 [ [H7_21 H7_22] H7_3]].
+         pose proof (PreCTX_rec_helper l l2 C Γ e p [] H2 ltac:(constructor) H3 H9 H7_21).
+         simpl in H4. subst.
+         epose proof (P := H7_3 (plugc C (CReceive [] p0 CHole l2)) _). do 2 rewrite <- plug_assoc in P.
+         simpl in P. apply P. auto.
+        }
+    all: shelve.
+Unshelve.
+    9-10: rewrite (indexed_to_forall _ _ (PNil, ELit 0%Z)) in H;
+         rewrite (indexed_to_forall _ _ (PNil, ELit 0%Z)) in H0;
+         constructor; intros.
+    9-10: replace (ELit 0%Z) with (snd (PNil, ELit 0%Z)) by auto.
+    9-10: replace 0 with ((fst >>> pat_vars) (PNil, ELit 0%Z)) by auto.
+    9-10: do 2 rewrite map_nth.
+    9: apply H in H2. 10: apply H0 in H2. 9-10: break_match_hyp; apply H2.
+  2-3, 6-7: exact (ELit 0%Z).
+  apply alpha_eval in H4; apply alpha_eval; rewrite default_context in *;
+       simpl in *; rewrite map_const in *; rewrite <- H; auto.
+
+  apply alpha_eval. apply alpha_eval in HC_e2. rewrite default_context in *. exact HC_e2.
+
+  apply alpha_eval. apply alpha_eval in HC_e2. rewrite default_context in *.
+  simpl in *; rewrite map_const in *; rewrite <- H; auto.
+
+  eapply plugc_preserves_scope_exp. exact H2. constructor. constructor.
+  intros. inversion H5.
+  intros. rewrite (indexed_to_forall _ _ (PNil, ELit 0%Z)) in H0.
+  specialize (H0 (S i) ltac:(simpl;lia)).
+  simpl in H0.
+  replace (ELit 0%Z) with (snd (PNil, ELit 0%Z)) by auto.
+  replace 0 with ((fst >>> pat_vars) (PNil, ELit 0%Z)) by auto.
+  do 2 rewrite map_nth.
+  break_match_hyp; cbn. auto.
+Qed.
+
+Lemma CTX_IsCtxRel : IsCtxRel CTX.
+Proof.
+  unfold IsCtxRel.
+  split.
+  - apply CTX_IsPreCtxRel.
+  - intros.
+    eapply CTX_bigger; eauto.
+Qed.
+
+Global Hint Resolve CTX_IsCtxRel : core.
+Global Hint Resolve CTX_IsPreCtxRel : core.
+
+Corollary CIU_implies_CTX :
+  forall Γ e1 e2, CIU_open Γ e1 e2 -> CTX Γ e1 e2.
+Proof.
+  intros. eapply CTX_bigger. 2: exact H. apply CIU_IsPreCtxRel.
+Qed.
+
+Global Hint Resolve CIU_implies_CTX : core.
+
+Lemma exists_CTX : exists R, IsCtxRel R.
+Proof.
+  exists CTX.
+  apply CTX_IsCtxRel.
+Qed.
+
+
+
+
+Lemma CIU_beta_value : forall {Γ e2 x v},
+    EXP S Γ ⊢ e2 -> VAL Γ ⊢ v ->
+    (CIU_open Γ e2.[v/] (ELet x v e2) /\ 
+     CIU_open Γ (ELet x v e2) e2.[v/]).
+Proof.
+  unfold CIU_open.
+  intros.
+  unfold CIU.
+  intuition idtac.
+  1,5: apply -> subst_preserves_scope_exp; try eassumption;
+    apply -> subst_preserves_scope_exp; eauto.
+  1,3: simpl; constructor; [ constructor; apply -> subst_preserves_scope_val; eauto |
+                             apply -> subst_preserves_scope_exp; eauto ].
+  destruct H3. exists (S (S x0)). simpl. apply term_let.
+  pose proof (subst_preserves_scope_val v Γ). destruct H4.
+  clear H5. specialize (H4 H0 0 ξ H1). constructor; auto.
+  rewrite subst_comp, subst_extend.
+  now rewrite subst_comp, scons_substcomp, substcomp_id_l in H3.
+
+  destruct H3. simpl in H3. inversion H3; try inversion_is_value. subst.
+  pose proof (subst_preserves_scope_val v Γ). destruct H4.
+  clear H5. specialize (H4 H0 0 ξ H1).
+  inversion H9; subst.
+  rewrite subst_comp, subst_extend in H12.
+  rewrite subst_comp, scons_substcomp, substcomp_id_l. eexists. exact H12.
+
+  all: rewrite <- H5 in H4; inversion H4.
+Qed.
+
+Lemma CTX_closed_under_substitution : forall {Γ e1 e2 v R},
+    IsCtxRel R ->
+    VAL Γ ⊢ v ->
+    R (S Γ) e1 e2 ->
+    R Γ e1.[v/] e2.[v/].
+Proof.
+  intros Γ e1 e2 v R HCtx Hscope_v HCtx_e1e2.
+  destruct HCtx as [HCtx Hbiggest].
+  destruct HCtx as [Rscope [Radequate [Rrefl [Rtrans [RFun [RApp [RLet [RLetRec [RPlus RIf]]]]]]]]].
+  destruct (Rscope _ _ _ HCtx_e1e2) as [Hscope_e1 Hscope_e2].
+  epose proof (@CIU_beta_value Γ e1 "X"%string v Hscope_e1 _).
+  epose proof (@CIU_beta_value Γ e2 "X"%string v Hscope_e2 _).
+  destruct H as [? _].
+  destruct H0 as [_ ?].
+  apply CIU_iff_Erel in H.
+  apply CIU_iff_Erel in H0.
+  apply Hbiggest in H; auto using Erel_IsPreCtxRel.
+  apply Hbiggest in H0; auto using Erel_IsPreCtxRel.
+  eapply Rtrans in H.
+  eapply H.
+  eapply Rtrans; revgoals.
+  eapply H0.
+  apply RLet.
+  1-2: constructor; auto.
+  1-2: auto.
+  apply Rrefl. now constructor.
+  auto.
+Unshelve.
+  1-2: auto.
+Qed.
+
+Theorem CIU_IsCtxRel : IsCtxRel CIU_open.
+Proof.
+  destruct exists_CTX as [R' HR'].
+  eapply bigger_implies_IsCtxRel. 2: eauto using CIU_IsPreCtxRel. apply CTX_IsCtxRel.
+  induction Γ; revgoals.
+  - unfold CIU_open.
+    intros.
+    pose proof (H0 0 ltac:(lia)). break_match_hyp. 2: inversion H1.
+    replace e1.[ξ] with e1.[e/].[(fun n => n + 1) >>> ξ]; revgoals.
+    {
+      rewrite subst_comp. rewrite scons_substcomp_core.
+      rewrite (vclosed_ignores_sub e); auto.
+      rewrite <- substcomp_scons, idsubst_up, substcomp_id_l.
+      now rewrite subst_ren_scons.
+    }
+    replace e2.[ξ] with e2.[e/].[(fun n => n + 1) >>> ξ]; revgoals.
+    {
+      rewrite subst_comp. rewrite scons_substcomp_core.
+      rewrite (vclosed_ignores_sub e); auto.
+      rewrite <- substcomp_scons, idsubst_up, substcomp_id_l.
+      now rewrite subst_ren_scons.
+    }
+    apply IHΓ.
+    apply CTX_closed_under_substitution; auto; revgoals.
+    + specialize (H0 0 ltac:(lia)).
+      simpl. replace e with (e.[idsubst]) by auto.
+      apply -> subst_preserves_scope_val; eauto. intro. intros. inversion H2.
+    + unfold subscoped.
+      intros. apply H0. lia.
+  - unfold CIU_open.
+    intros.
+    unfold CIU.
+    intuition idtac.
+    + apply -> subst_preserves_scope_exp; eauto. destruct HR'.
+      eapply H1 with (e1:=e1) (e2:=e2). apply H2 in H; auto.
+    + apply -> subst_preserves_scope_exp; eauto 3. destruct HR'.
+      eapply H1 with (e1:=e1) (e2:=e2); eauto 3.
+    + replace e1.[ξ] with e1 in H2; revgoals.
+      { replace ξ with (upn 0 ξ) by auto.
+        rewrite escoped_ignores_sub; auto. destruct HR'.
+        eapply H3 with (e1:=e1) (e2:=e2); eauto.
+      }
+      replace e2.[ξ] with e2; revgoals.
+      { replace ξ with (upn 0 ξ) by auto.
+        rewrite escoped_ignores_sub; auto. destruct HR'.
+        eapply H3 with (e1:=e1) (e2:=e2); eauto.
+      }
+      clear H0.
+      generalize dependent e2. generalize dependent e1. generalize dependent F.
+      induction F; intros.
+      * destruct HR'. destruct H, H. apply (H4 CHole); auto. constructor.
+      * inversion H1. subst.
+        assert (EXPCLOSED e1) as EC1 by apply H.
+        assert (EXPCLOSED e2) as EC2 by apply H.
+        apply put_back in H2; auto. destruct H2. apply put_back_rev; auto.
+        eapply IHF; auto. exists x. exact H0.
+        destruct HR'. inversion H. clear H6.
+        destruct a; inversion H4; subst.
+        -- simpl. apply CTX_IsPreCtxRel; auto. apply forall_biforall_refl.
+           apply Forall_forall. intros. apply CTX_refl. rewrite Forall_forall in H8.
+           now apply H8.
+        -- simpl. apply CTX_IsPreCtxRel; auto.
+           ++ apply Forall_app. split; auto. eapply Forall_impl. 2: exact H12.
+              intros. now constructor.
+           ++ apply Forall_app. split; auto. eapply Forall_impl. 2: exact H12.
+              intros. now constructor.
+           ++ apply CTX_refl. now constructor.
+           ++ apply biforall_app. 2: constructor; auto.
+              all: apply forall_biforall_refl; apply Forall_forall; 
+                   intros; apply CTX_refl; rewrite Forall_forall in H11, H12.
+              constructor. now apply H12.
+              now apply H11.
+        -- simpl. apply CTX_IsPreCtxRel; auto. now apply CTX_refl.
+        -- simpl. apply CTX_IsPreCtxRel; auto.
+           1-2: now rewrite Nat.add_0_r. 1-2: apply CTX_refl; auto; now rewrite Nat.add_0_r.
+        -- simpl. apply CTX_IsPreCtxRel; auto. now apply CTX_refl.
+        -- simpl. apply CTX_IsPreCtxRel; auto.
+           apply CTX_refl.
+           all: apply scoped_val; auto.
+        -- simpl. apply CTX_IsPreCtxRel; auto. apply forall_biforall_refl.
+           apply Forall_forall. intros. apply CTX_refl. rewrite Forall_forall in H8.
+           now apply H8.
+        -- simpl. apply CTX_IsPreCtxRel; auto.
+           ++ apply Forall_app. split; auto. eapply Forall_impl. 2: exact H12.
+              intros. now constructor.
+           ++ apply Forall_app. split; auto. eapply Forall_impl. 2: exact H12.
+              intros. now constructor.
+           ++ apply CTX_refl. now constructor.
+           ++ apply biforall_app. 2: constructor; auto.
+              all: apply forall_biforall_refl; apply Forall_forall; 
+                   intros; apply CTX_refl; rewrite Forall_forall in H11, H12.
+              constructor. now apply H12.
+              now apply H11.
+Qed.
+
+Theorem Erel_IsCtxRel : IsCtxRel Erel_open.
+Proof.
+  unfold IsCtxRel.
+  split.
+  apply Erel_IsPreCtxRel.
+  intros.
+  apply CIU_iff_Erel.
+  pose proof CIU_IsCtxRel.
+  unfold IsCtxRel in H1.
+  destruct H1.
+  eapply H2; eauto.
+Qed.
+
+Corollary CTX_implies_CIU :
+  forall e1 e2 Γ, CTX Γ e1 e2 -> CIU_open Γ e1 e2.
+Proof.
+  intros. eapply CIU_IsCtxRel. 2: exact H. auto.
+Qed.
+
+Global Hint Resolve CTX_implies_CIU : core.
+
+Corollary CIU_iff_CTX :
+  forall e1 e2 Γ, CTX Γ e1 e2 <-> CIU_open Γ e1 e2.
+Proof.
+  intros. split; auto.
+Qed.
+
+Corollary Erel_iff_CTX :
+  forall e1 e2 Γ, CTX Γ e1 e2 <-> Erel_open Γ e1 e2.
+Proof.
+  intros. split; intros.
+  * apply CIU_iff_Erel. auto.
+  * apply CIU_iff_Erel in H. auto.
+Qed.
+
+Corollary CTX_eval : forall e1 v,
+  EXPCLOSED e1 ->
+  ⟨ [], e1 ⟩ -->* v -> CTX 0 e1 v /\ CTX 0 v e1.
+Proof.
+  intros. split; apply CIU_iff_CTX; intro; intros.
+  rewrite eclosed_ignores_sub, vclosed_ignores_sub.
+  4: rewrite vclosed_ignores_sub, eclosed_ignores_sub.
+  1, 4: pose proof (CIU_eval _ _ H H0). all: auto. 1-2: apply H2.
+  all: apply step_any_closedness in H0; auto; constructor.
+Qed.
+
+
+
+
+
+
+
+
+
+
+
+
+
+
+
+
+
+
+
+
+
+
+
+
+
+
+
+
+
+
+
+
+
+
+
+
+
+
+
+
+
+
+
+
+
 
 
 Inductive Ctx :=
@@ -402,7 +1398,40 @@ Inductive Ctx :=
 | CTuple   (l : list Exp) (c : Ctx) (l' : list Exp)
 | CMap1    (l : list (Exp * Exp)) (c : Ctx) (e2 : Exp) (l' : list (Exp * Exp))
 | CMap2    (l : list (Exp * Exp)) (e1 : Exp) (c : Ctx) (l' : list (Exp * Exp))
-| CCall    (m f : string)    (l : list Exp) (c : Ctx) (l' : list Exp)
+| CCallMod (c : Ctx) (f : Exp) (l : list Exp)
+| CCallFun (m : Exp) (c : Ctx) (l : list Exp)
+| CCallParam (m f : Exp)    (l : list Exp) (c : Ctx) (l' : list Exp)
+| CPrimOp  (f : string)    (l : list Exp) (c : Ctx) (l' : list Exp)
+| CApp1    (c : Ctx) (l : list Exp)
+| CApp2    (exp: Exp) (l : list Exp) (c : Ctx) (l' : list Exp)
+| CCase1   (c : Ctx) (l : list ((list Pat) * Exp * Exp))
+| CCase2   (e : Exp) (l : list ((list Pat) * Exp * Exp)) (lp : (list Pat)) (c : Ctx) (e2 : Exp) (l' : list ((list Pat) * Exp * Exp))
+| CCase3   (e : Exp) (l : list ((list Pat) * Exp * Exp)) (lp : (list Pat)) (e1 : Exp) (c : Ctx) (l' : list ((list Pat) * Exp * Exp))
+| CLet1    (l : nat) (c : Ctx) (e2 : Exp)
+| CLet2    (l : nat) (e1: Exp) (c : Ctx)
+| CSeq1    (c : Ctx) (e2 : Exp)
+| CSeq2    (e1 : Exp) (c : Ctx)
+| CLetRec1 (l : list (nat * Exp)) (n : nat) (c : Ctx) (l' : list (nat * Exp)) (e : Exp)
+| CLetRec2 (l : list (nat * Exp)) (c : Ctx)
+| CTry1    (c : Ctx) (vl1 : nat) (e2 : Exp) (vl2 : nat) (e3 : Exp)
+| CTry2    (e1 : Exp) (vl1 : nat) (c : Ctx) (vl2 : nat) (e3 : Exp)
+| CTry3    (e1 : Exp) (vl1 : nat) (e2 : Exp) (vl2 : nat) (c : Ctx)
+.
+
+
+
+Inductive Ctx :=
+| CHole
+| CFun     (vl : nat) (c : Ctx)
+| CValues  (el : list Exp) (c : Ctx) (el' : list Exp)
+| CCons1   (c : Ctx) (tl : Exp)
+| CCons2   (hd : Exp) (c : Ctx)
+| CTuple   (l : list Exp) (c : Ctx) (l' : list Exp)
+| CMap1    (l : list (Exp * Exp)) (c : Ctx) (e2 : Exp) (l' : list (Exp * Exp))
+| CMap2    (l : list (Exp * Exp)) (e1 : Exp) (c : Ctx) (l' : list (Exp * Exp))
+| CCallMod (c : Ctx) (f : Exp) (l : list Exp)
+| CCallFun (m : Exp) (c : Ctx) (l : list Exp)
+| CCallParam (m f : Exp)    (l : list Exp) (c : Ctx) (l' : list Exp)
 | CPrimOp  (f : string)    (l : list Exp) (c : Ctx) (l' : list Exp)
 | CApp1    (c : Ctx) (l : list Exp)
 | CApp2    (exp: Exp) (l : list Exp) (c : Ctx) (l' : list Exp)
@@ -430,7 +1459,10 @@ match C with
 | CTuple  l c l'     => EExp ( ETuple (l ++ [(plug c p)] ++ l') )
 | CMap1   l c e2 l'  => EExp ( EMap (l ++ [((plug c p), e2)] ++ l') )
 | CMap2   l e1 c l'  => EExp ( EMap (l ++ [(e1, (plug c p))] ++ l') )
-| CCall   m f l c l'   => EExp ( ECall m f (l ++ [(plug c p)] ++ l') )
+| CCallMod c f l     => EExp ( ECall (plug c p) f l )
+| CCallFun m c l     => EExp ( ECall m (plug c p) l )
+| CCallParam   m f l c l'
+                     => EExp ( ECall m f (l ++ [(plug c p)] ++ l') )
 | CPrimOp f l c l'   => EExp ( EPrimOp f (l ++ [(plug c p)] ++ l') )
 | CApp1   c l        => EExp ( EApp (plug c p) l )
 | CApp2   exp l c l' => EExp ( EApp exp (l ++ [(plug c p)] ++ l') )
@@ -458,7 +1490,10 @@ match C with
 | CTuple  l c l'    => CTuple l (plugc c p) l'
 | CMap1   l c e2 l' => CMap1 l (plugc c p) e2 l'
 | CMap2   l e1 c l' => CMap2 l e1 (plugc c p) l'
-| CCall   m f l c l'  => CCall m f l (plugc c p) l'
+| CCallMod c f l    => CCallMod (plugc c p) f l
+| CCallFun m c l    => CCallFun m (plugc c p) l
+| CCallParam m f l c l' 
+                    => CCallParam m f l (plugc c p) l'
 | CPrimOp f l c l'  => CPrimOp f l (plugc c p) l'
 | CApp1   c l       => CApp1 (plugc c p) l
 | CApp2   exp l c l' => CApp2 exp l (plugc c p) l'
@@ -485,7 +1520,7 @@ Proof.
     intros;
     cbn;
     auto;
-    rewrite IHC1;
+    try rewrite IHC1;
     auto.
 Qed.
 
@@ -536,11 +1571,25 @@ Inductive EECtxScope (Γh : nat) : nat -> Ctx -> Prop :=
   EECTX Γh ⊢ c ∷ Γ ->
   EECTX Γh ⊢ (CMap2 l e1 c l') ∷ Γ
 
-| CEScope_CCall : forall Γ m f l c l',
+| CEScope_CCallMod : forall Γ c f l,
+  EECTX Γh ⊢ c ∷ Γ ->
+  EXP Γ ⊢ f ->
+  Forall (fun e => EXP Γ ⊢ e) l ->
+  EECTX Γh ⊢ CCallMod c f l ∷ Γ
+
+| CEScope_CCallFun : forall Γ m c l,
+  EXP Γ ⊢ m ->
+  EECTX Γh ⊢ c ∷ Γ ->
+  Forall (fun e => EXP Γ ⊢ e) l ->
+  EECTX Γh ⊢ CCallFun m c l ∷ Γ
+
+| CEScope_CCallParam : forall Γ m f l c l',
+  EXP Γ ⊢ m ->
+  EXP Γ ⊢ f ->
   Forall (fun e => EXP Γ ⊢ e) l ->
   EECTX Γh ⊢ c ∷ Γ ->
   Forall (fun e => EXP Γ ⊢ e) l' ->
-  EECTX Γh ⊢ (CCall m f l c l') ∷ Γ
+  EECTX Γh ⊢ (CCallParam m f l c l') ∷ Γ
 
 | CEScope_CPrimOp : forall Γ f l c l',
   Forall (fun e => EXP Γ ⊢ e) l ->
@@ -671,8 +1720,13 @@ Proof.
       intros. apply indexed_to_forall. 2: auto.
       rewrite map_app. apply Forall_app; split; auto.
       constructor; auto. simpl. now apply IHC. now rewrite map_length.
+  * do 2 constructor. apply indexed_to_forall. exact H7.
+    all: auto.
+  * do 2 constructor. apply indexed_to_forall. exact H7.
+    all: auto.
   * do 2 constructor. apply indexed_to_forall.
     apply Forall_app; split; auto.
+    all: auto.
   * do 2 constructor. apply indexed_to_forall.
     apply Forall_app; split; auto.
   * do 2 constructor. now apply IHC.
@@ -778,174 +1832,185 @@ Proof.
   { clear H0 H1.
     induction C;
       intros;
-      inversion H0;
-      subst;
+      inv H0;
       cbn;
       try solve_inversion;
       auto.
     - apply RFun. reflexivity.
       1-2: eapply plug_preserves_scope_exp; eauto.
       apply IHC; auto.
-    - apply RValues. do 2 rewrite app_length. reflexivity.
-      1-2: inv H0; apply Forall_app; split; auto; constructor; auto.
+    - apply RValues.
+      1-2: apply Forall_app; split; auto; constructor; auto.
       1-2: eapply plug_preserves_scope_exp; eauto.
       apply biforall_app. 2: constructor.
       + apply forall_biforall_refl, Forall_forall. intros.
-        rewrite Forall_forall in H5. apply Rrefl. now apply H5 in H1.
+        rewrite Forall_forall in H5. apply Rrefl. now apply H5 in H0.
       + apply IHC; auto.
       + apply forall_biforall_refl, Forall_forall. intros.
-        rewrite Forall_forall in H7. apply Rrefl. now apply H7 in H1.
+        rewrite Forall_forall in H7. apply Rrefl. now apply H7 in H0.
     - apply RCons; auto.
-      + eapply @plug_preserves_scope_exp with (e := e1) in H0; eauto 2.
-        simpl in H0. inv H0. now inv H3.
-      + eapply @plug_preserves_scope_exp with (e := e2) in H0; eauto 2.
-        simpl in H0. inv H0. now inv H3.
+      + eapply @plug_preserves_scope_exp with (e := e1) in H4; eauto 2.
+      + eapply @plug_preserves_scope_exp with (e := e2) in H4; eauto 2.
     - apply RCons; auto.
-      + eapply @plug_preserves_scope_exp with (e := e1) in H0; eauto 2.
-        simpl in H0. inv H0. now inv H3.
-      + eapply @plug_preserves_scope_exp with (e := e2) in H0; eauto 2.
-        simpl in H0. inv H0. now inv H3.
+      + eapply @plug_preserves_scope_exp with (e := e1) in H5; eauto 2.
+      + eapply @plug_preserves_scope_exp with (e := e2) in H5; eauto 2.
+    - apply RTuple; auto.
+      1-2: apply Forall_app; split; auto; constructor; auto.
+      1-2: eapply plug_preserves_scope_exp; eauto.
+      apply biforall_app. 2: constructor.
+      + apply forall_biforall_refl, Forall_forall. intros.
+        rewrite Forall_forall in H5. apply Rrefl. now apply H5 in H0.
+      + apply IHC; auto.
+      + apply forall_biforall_refl, Forall_forall. intros.
+        rewrite Forall_forall in H7. apply Rrefl. now apply H7 in H0.
+    - apply RMap; auto.
+      1-2: apply Forall_app; split; auto; constructor; auto.
+      1-2: split; simpl; try eapply plug_preserves_scope_exp; eauto.
+      apply biforall_app. 2: constructor.
+      + apply forall_biforall_refl, Forall_forall. intros.
+        rewrite Forall_forall in H6. destruct x; split;
+        apply Rrefl; apply H6 in H0; now destruct H0.
+      + split; auto.
+      + apply forall_biforall_refl, Forall_forall. intros.
+        rewrite Forall_forall in H7. destruct x; split;
+        apply Rrefl; apply H7 in H0; now destruct H0.
+    - apply RMap; auto.
+      1-2: apply Forall_app; split; auto; constructor; auto.
+      1-2: split; simpl; try eapply plug_preserves_scope_exp; eauto.
+      apply biforall_app. 2: constructor.
+      + apply forall_biforall_refl, Forall_forall. intros.
+        rewrite Forall_forall in H6. destruct x; split;
+        apply Rrefl; apply H6 in H0; now destruct H0.
+      + split; auto.
+      + apply forall_biforall_refl, Forall_forall. intros.
+        rewrite Forall_forall in H7. destruct x; split;
+        apply Rrefl; apply H7 in H0; now destruct H0.
+    - apply RCall; auto.
+      1-2: eapply plug_preserves_scope_exp; eauto.
+      apply forall_biforall_refl, Forall_forall. intros.
+      rewrite Forall_forall in H7. now apply Rrefl, H7.
+    - apply RCall; auto.
+      1-2: eapply plug_preserves_scope_exp; eauto.
+      apply forall_biforall_refl, Forall_forall. intros.
+      rewrite Forall_forall in H7. now apply Rrefl, H7.
+    - apply RCall; auto.
+      1-2: apply Forall_app; split; auto; constructor; auto.
+      1-2: simpl; try eapply plug_preserves_scope_exp; eauto.
+      apply biforall_app. 2: constructor.
+      + apply forall_biforall_refl, Forall_forall. intros.
+        rewrite Forall_forall in H9.
+        apply Rrefl. now apply H9 in H0.
+      + now apply IHC.
+      + apply forall_biforall_refl, Forall_forall. intros.
+        rewrite Forall_forall in H11.
+        apply Rrefl. now apply H11 in H0.
+    - apply RPrimOp; auto.
+      1-2: apply Forall_app; split; auto; constructor; auto.
+      1-2: simpl; try eapply plug_preserves_scope_exp; eauto.
+      apply biforall_app. 2: constructor.
+      + apply forall_biforall_refl, Forall_forall. intros.
+        rewrite Forall_forall in H5.
+        apply Rrefl. now apply H5 in H0.
+      + now apply IHC.
+      + apply forall_biforall_refl, Forall_forall. intros.
+        rewrite Forall_forall in H8.
+        apply Rrefl. now apply H8 in H0.
     - apply RApp; auto.
-      + eapply @plug_preserves_scope_exp with (e := e1) in H0; eauto 2.
-        simpl in H0. inversion H0. subst. auto. inversion H1.
-      + eapply @plug_preserves_scope_exp with (e := e2) in H0; eauto 2.
-        simpl in H0. inversion H0. subst. auto. inversion H1.
+      + eapply @plug_preserves_scope_exp with (e := e1) in H4; eauto 2.
+      + eapply @plug_preserves_scope_exp with (e := e2) in H4; eauto 2.
       + apply forall_biforall_refl.
         apply Forall_forall. rewrite Forall_forall in H5. intros. apply Rrefl. auto.
     - apply RApp; auto.
-      + rewrite indexed_to_forall. intros.
-        epose (nth_possibilities _ _ _ _ H1). destruct o.
-        * destruct H2. rewrite H2 in *. rewrite indexed_to_forall in H7. apply H7. auto.
-        * destruct H2. rewrite H2 in *. rewrite indexed_to_forall in H8.
-          remember (i - length l1) as i'. destruct i'.
-          -- simpl. eapply @plug_preserves_scope_exp with (e := e1) in H0; eauto 2.
-             simpl in H0. inversion H0. subst. 2: inversion H4.
-             epose (H11 (length l1) _). rewrite nth_middle in e. auto.
-             Unshelve. 1-2: exact (ELit 0%Z). rewrite app_length. lia.
-          -- simpl. apply H8. simpl in H3. lia.
-      + rewrite indexed_to_forall. intros.
-        epose (nth_possibilities _ _ _ _ H1). destruct o.
-        * destruct H2. rewrite H2 in *. rewrite indexed_to_forall in H7. apply H7. auto.
-        * destruct H2. rewrite H2 in *. rewrite indexed_to_forall in H8.
-          remember (i - length l1) as i'. destruct i'.
-          -- simpl. eapply @plug_preserves_scope_exp with (e := e2) in H0; eauto 2.
-             simpl in H0. inversion H0. subst. 2: inversion H4.
-             epose (H11 (length l1) _). rewrite nth_middle in e. auto.
-             Unshelve. 1-2: exact (ELit 0%Z). rewrite app_length. lia.
-          -- simpl. apply H8. simpl in H3. lia.
-      + apply biforall_app. 2: constructor.
-        ** apply forall_biforall_refl, Forall_forall. rewrite Forall_forall in H7. auto.
-        ** simpl. apply IHC. auto.
-        ** apply forall_biforall_refl, Forall_forall. rewrite Forall_forall in H8. auto.
-    - apply RLet; auto.
-      + eapply @plug_preserves_scope_exp with (e := e1) in H0; eauto 2.
-        simpl in H0. inversion H0. auto. inversion H1.
-      + eapply @plug_preserves_scope_exp with (e := e2) in H0; eauto 2.
-        simpl in H0. inversion H0. auto. inversion H1.
-    - apply RLet; auto.
-      + eapply @plug_preserves_scope_exp with (e := e1) in H0; eauto 2.
-        simpl in H0. inversion H0. auto. inversion H1.
-      + eapply @plug_preserves_scope_exp with (e := e2) in H0; eauto 2.
-        simpl in H0. inversion H0. auto. inversion H1.
-    - apply RLetRec; auto.
-      + eapply @plug_preserves_scope_exp with (e := e1) in H0; eauto 2.
-        simpl in H0. inversion H0. auto. inversion H1.
-      + eapply @plug_preserves_scope_exp with (e := e2) in H0; eauto 2.
-        simpl in H0. inversion H0. auto. inversion H1.
-    - apply RLetRec; auto.
-      + eapply @plug_preserves_scope_exp with (e := e1) in H0; eauto 2.
-        simpl in H0. inversion H0. auto. inversion H1.
-      + eapply @plug_preserves_scope_exp with (e := e2) in H0; eauto 2.
-        simpl in H0. inversion H0. auto. inversion H1.
+      1-2: apply Forall_app; split; auto; constructor; auto.
+      1-2: simpl; try eapply plug_preserves_scope_exp; eauto.
+      apply biforall_app. 2: constructor.
+      + apply forall_biforall_refl, Forall_forall. intros.
+        rewrite Forall_forall in H7.
+        apply Rrefl. now apply H7 in H0.
+      + now apply IHC.
+      + apply forall_biforall_refl, Forall_forall. intros.
+        rewrite Forall_forall in H9.
+        apply Rrefl. now apply H9 in H0.
     - apply RCase; auto.
-      + eapply @plug_preserves_scope_exp with (e := e1) in H0; eauto 2.
-        simpl in H0. inversion H0. auto. inversion H1.
-      + eapply @plug_preserves_scope_exp with (e := e2) in H0; eauto 2.
-        simpl in H0. inversion H0. auto. inversion H1.
-    - apply RCase; auto.
-      + eapply @plug_preserves_scope_exp with (e := e1) in H0; eauto 2.
-        simpl in H0. inversion H0. auto. inversion H1.
-      + eapply @plug_preserves_scope_exp with (e := e2) in H0; eauto 2.
-        simpl in H0. inversion H0. auto. inversion H1.
-    - apply RCase; auto.
-      + eapply @plug_preserves_scope_exp with (e := e1) in H0; eauto 2.
-        simpl in H0. inversion H0. auto. inversion H1.
-      + eapply @plug_preserves_scope_exp with (e := e2) in H0; eauto 2.
-        simpl in H0. inversion H0. auto. inversion H1.
-    - apply RCons; auto.
-      + eapply @plug_preserves_scope_exp with (e := e1) in H0; eauto 2.
-        simpl in H0. inversion H0. auto. inversion H1.
-      + eapply @plug_preserves_scope_exp with (e := e2) in H0; eauto 2.
-        simpl in H0. inversion H0. auto. inversion H1.
-    - apply RCons; auto.
-      + eapply @plug_preserves_scope_exp with (e := e1) in H0; eauto 2.
-        simpl in H0. inversion H0. auto. inversion H1.
-      + eapply @plug_preserves_scope_exp with (e := e2) in H0; eauto 2.
-        simpl in H0. inversion H0. auto. inversion H1.
-    - apply RBIF; auto.
-      + eapply @plug_preserves_scope_exp with (e := e1) in H0; eauto 2.
-        simpl in H0. inversion H0. subst. auto. inversion H1.
-      + eapply @plug_preserves_scope_exp with (e := e2) in H0; eauto 2.
-        simpl in H0. inversion H0. subst. auto. inversion H1.
+      + eapply @plug_preserves_scope_exp with (e := e1) in H4; eauto 2.
+      + eapply @plug_preserves_scope_exp with (e := e2) in H4; eauto 2.
       + apply forall_biforall_refl.
-        apply Forall_forall. rewrite Forall_forall in H5. intros. apply Rrefl. auto.
-    - apply RBIF; auto.
-      + rewrite indexed_to_forall. intros.
-        epose (nth_possibilities _ _ _ _ H1). destruct o.
-        * destruct H2. rewrite H2 in *. rewrite indexed_to_forall in H7. apply H7. auto.
-        * destruct H2. rewrite H2 in *. rewrite indexed_to_forall in H8.
-          remember (i - length l1) as i'. destruct i'.
-          -- simpl. eapply @plug_preserves_scope_exp with (e := e1) in H0; eauto 2.
-             simpl in H0. inversion H0. subst. 2: inversion H4.
-             epose (H11 (length l1) _). rewrite nth_middle in e. auto.
-             Unshelve. 1-2: exact (ELit 0%Z). rewrite app_length. lia.
-          -- simpl. apply H8. simpl in H3. lia.
-      + rewrite indexed_to_forall. intros.
-        epose (nth_possibilities _ _ _ _ H1). destruct o.
-        * destruct H2. rewrite H2 in *. rewrite indexed_to_forall in H7. apply H7. auto.
-        * destruct H2. rewrite H2 in *. rewrite indexed_to_forall in H8.
-          remember (i - length l1) as i'. destruct i'.
-          -- simpl. eapply @plug_preserves_scope_exp with (e := e2) in H0; eauto 2.
-             simpl in H0. inversion H0. subst. 2: inversion H4.
-             epose (H11 (length l1) _). rewrite nth_middle in e. auto.
-             Unshelve. 1-2: exact (ELit 0%Z). rewrite app_length. lia.
-          -- simpl. apply H8. simpl in H3. lia.
-      + apply biforall_app. 2: constructor.
-        ** apply forall_biforall_refl, Forall_forall. rewrite Forall_forall in H7. auto.
-        ** simpl. apply IHC. auto.
-        ** apply forall_biforall_refl, Forall_forall. rewrite Forall_forall in H8. auto.
-    - apply RReceive; auto.
-      + apply Forall_app; split. 2: constructor.
-        1,3: rewrite (indexed_to_forall _ _ (PNil, ELit 0%Z)); intros.
-        * apply H7 in H1.
-          replace (ELit 0%Z) with (snd (PNil, ELit 0%Z)) in H1 by auto.
-          replace 0 with ((fst >>> pat_vars) (PNil, ELit 0%Z)) in H1 by auto.
-          do 2 rewrite map_nth in H1. break_match_goal. exact H1.
-        * apply H8 in H1.
-          replace (ELit 0%Z) with (snd (PNil, ELit 0%Z)) in H1 by auto.
-          replace 0 with ((fst >>> pat_vars) (PNil, ELit 0%Z)) in H1 by auto.
-          do 2 rewrite map_nth in H1. break_match_goal. exact H1.
-        * eapply @plug_preserves_scope_exp with (e := e1) in H5; eauto 2.
-      + apply Forall_app; split. 2: constructor.
-        1,3: rewrite (indexed_to_forall _ _ (PNil, ELit 0%Z)); intros.
-        * apply H7 in H1.
-          replace (ELit 0%Z) with (snd (PNil, ELit 0%Z)) in H1 by auto.
-          replace 0 with ((fst >>> pat_vars) (PNil, ELit 0%Z)) in H1 by auto.
-          do 2 rewrite map_nth in H1. break_match_goal. exact H1.
-        * apply H8 in H1.
-          replace (ELit 0%Z) with (snd (PNil, ELit 0%Z)) in H1 by auto.
-          replace 0 with ((fst >>> pat_vars) (PNil, ELit 0%Z)) in H1 by auto.
-          do 2 rewrite map_nth in H1. break_match_goal. exact H1.
-        * eapply @plug_preserves_scope_exp with (e := e2) in H5; eauto 2.
-      + apply biforall_app. 2: constructor.
-        * clear H0. (* biforall_refl not sufficient, bc preconditions *)
-          induction l1; constructor; auto. 2: apply IHl1; auto.
-          destruct a. split; auto. apply Rrefl. apply (H7 0). simpl. lia.
-          intros. apply (H7 (S i)). simpl. lia.
-        * split; auto.
-        * clear H0. induction l2; constructor; auto. 2: apply IHl2; auto.
-          destruct a. split; auto. apply Rrefl. apply (H8 0). simpl. lia.
-          intros. apply (H8 (S i)). simpl. lia.
+        apply Forall_forall. rewrite Forall_forall in H5. intros.
+        destruct x, p. split. 2: split. reflexivity.
+        all: apply Rrefl; now apply H5 in H0.
+    - apply RCase; auto.
+      1-2: apply Forall_app; split; auto; constructor; auto.
+      1-2: simpl; split; try eapply plug_preserves_scope_exp; eauto.
+      apply biforall_app. 2: constructor.
+      + apply forall_biforall_refl, Forall_forall. intros.
+        rewrite Forall_forall in H10. destruct x, p. split. 2: split.
+        reflexivity.
+        all: apply Rrefl; now apply H10 in H0.
+      + split; auto.
+      + apply forall_biforall_refl, Forall_forall. intros.
+        rewrite Forall_forall in H11. destruct x, p. split. 2: split.
+        reflexivity.
+        all: apply Rrefl; now apply H11 in H0.
+    - apply RCase; auto.
+      1-2: apply Forall_app; split; auto; constructor; auto.
+      1-2: simpl; split; try eapply plug_preserves_scope_exp; eauto.
+      apply biforall_app. 2: constructor.
+      + apply forall_biforall_refl, Forall_forall. intros.
+        rewrite Forall_forall in H10. destruct x, p. split. 2: split.
+        reflexivity.
+        all: apply Rrefl; now apply H10 in H0.
+      + split; auto.
+      + apply forall_biforall_refl, Forall_forall. intros.
+        rewrite Forall_forall in H11. destruct x, p. split. 2: split.
+        reflexivity.
+        all: apply Rrefl; now apply H11 in H0.
+    - apply RLet; auto.
+      + eapply @plug_preserves_scope_exp with (e := e1) in H4; eauto 2.
+      + eapply @plug_preserves_scope_exp with (e := e2) in H4; eauto 2.
+    - apply RLet; auto.
+      + eapply @plug_preserves_scope_exp with (e := e1) in H6; eauto 2.
+      + eapply @plug_preserves_scope_exp with (e := e2) in H6; eauto 2.
+    - apply RSeq; auto.
+      + eapply @plug_preserves_scope_exp with (e := e1) in H4; eauto 2.
+      + eapply @plug_preserves_scope_exp with (e := e2) in H4; eauto 2.
+    - apply RSeq; auto.
+      + eapply @plug_preserves_scope_exp with (e := e1) in H5; eauto 2.
+      + eapply @plug_preserves_scope_exp with (e := e2) in H5; eauto 2.
+    - apply RLetRec; auto.
+      + rewrite app_length. eauto.
+      + rewrite app_length. eauto.
+      + apply Forall_app. split. rewrite app_length. exact H6.
+        constructor. eapply plug_preserves_scope_exp. rewrite app_length.
+        exact H8. auto.
+        rewrite app_length. exact H9.
+      + apply Forall_app. split. rewrite app_length. exact H6.
+        constructor. eapply plug_preserves_scope_exp. rewrite app_length.
+        exact H8. auto.
+        rewrite app_length. exact H9.
+      + rewrite app_length in *. apply biforall_app. 2: constructor.
+        ** apply forall_biforall_refl, Forall_forall. intros.
+           rewrite Forall_forall in H6. destruct x. split. reflexivity.
+           apply Rrefl; now apply H6 in H0.
+        ** split; auto.
+        ** apply forall_biforall_refl, Forall_forall. intros.
+           rewrite Forall_forall in H9. destruct x. split. reflexivity.
+           apply Rrefl; now apply H9 in H0.
+      + apply Rrefl. rewrite app_length; auto.
+    - apply RLetRec; auto.
+      + eapply @plug_preserves_scope_exp with (e := e1) in H5; eauto 2.
+      + eapply @plug_preserves_scope_exp with (e := e2) in H5; eauto 2.
+      + apply forall_biforall_refl, Forall_forall. intros.
+        rewrite Forall_forall in H4. destruct x. split. reflexivity.
+        apply Rrefl; now apply H4 in H0.
+    - apply RTry; auto.
+      + eapply @plug_preserves_scope_exp with (e := e1) in H5; eauto 2.
+      + eapply @plug_preserves_scope_exp with (e := e2) in H5; eauto 2.
+    - apply RTry; auto.
+      + eapply @plug_preserves_scope_exp with (e := e1) in H8; eauto 2.
+      + eapply @plug_preserves_scope_exp with (e := e2) in H8; eauto 2.
+    - apply RTry; auto.
+      + eapply @plug_preserves_scope_exp with (e := e1) in H9; eauto 2.
+      + eapply @plug_preserves_scope_exp with (e := e2) in H9; eauto 2.
   }
   now apply H2.
 Qed.
@@ -955,5 +2020,449 @@ Proof.
   unfold CTX. intros. split; auto.
 Qed.
 
+Lemma CTX_IsPreCtxRel : IsPreCtxRel CTX.
+Proof.
+  unfold IsPreCtxRel.
+  intuition idtac;
+    try solve
+        [unfold CTX in H; intuition idtac
+        |inversion H; [|constructor]; apply H0].
+  * unfold Adequate.
+    intros.
+    unfold CTX in H.
+    intuition idtac.
+    - apply (H2 CHole); auto.
+      constructor.
+  * unfold IsReflexive.
+    intros.
+    unfold CTX.
+    intuition (auto using Rbar_le_refl).
+  * unfold Transitive.
+    intros.
+    unfold CTX in *.
+    intuition idtac.
+    auto.
+  * unfold CompatibleFun.
+    intros.
+    unfold CTX in *.
+    intuition auto.
+    specialize (H4 (plugc C (CFun vl' CHole))).
+    repeat rewrite <- plug_assoc in H4.
+    cbn in H4.
+    apply H4.
+    eapply plugc_preserves_scope_exp; eauto.
+    constructor. subst. constructor. now subst.
+  * unfold CompatibleValues.
+    intros. unfold CTX in *.
+    intuition auto.
+    1-2: do 2 constructor; rewrite <- indexed_to_forall; eassumption.
+    clear H H0. generalize dependent C. induction H1; intros.
+    - assumption.
+    - replace (plug C (° EValues (hd :: tl))) with
+              (plug (plugc C (CValues [] CHole tl)) hd) in H3 
+        by now rewrite <- plug_assoc.
+      destruct H. apply H0 in H3.
+      
+  * unfold CompatibleApp.
+    intros.
+    unfold CTX in *.
+    intuition auto.
+    1-2: rewrite indexed_to_forall in H, H0; constructor; auto.
+    clear H3 H7.
+    assert (EECTX Γ ⊢ plugc C (CAppFun CHole vals1) ∷ 0) as HC_e1.
+    { eapply plugc_preserves_scope_exp; eauto.
+      constructor; auto.
+      constructor.
+    }
+    apply H6 in HC_e1. 2: rewrite <- plug_assoc in *; simpl; auto.
+    apply biforall_length in H4 as LL. rewrite <- plug_assoc in HC_e1.
+    destruct vals1; intros.
+    - inversion H4. now subst.
+    - inversion H4. subst. destruct H9, H3. inversion H. inversion H0. subst.
+      assert (EECTX Γ ⊢ plugc C (CAppParam f2 [] CHole vals1) ∷ 0). {
+        eapply plugc_preserves_scope_exp; eauto.
+        constructor; auto.
+        constructor.
+      }
+      apply H7 in H10. 2: now rewrite <- plug_assoc.
+      replace (hd' :: tl') with ([] ++ [hd'] ++ tl') by auto.
+      eapply PreCTX_app_helper; eauto.
+      now rewrite plug_assoc.
+  * unfold CompatibleLet.
+    intros.
+    unfold CTX in *.
+    intuition auto.
+    clear H5 H9 H4 H8.
+    assert (EECTX Γ ⊢ plugc C (CLet1 x CHole e2) ∷ 0) as HC_e1.
+    { eapply plugc_preserves_scope_exp; eauto.
+      constructor; auto.
+      constructor.
+    }
+    assert (EECTX S Γ ⊢ plugc C (CLet2 x e1' CHole) ∷ 0) as HC_e2.
+    { eapply plugc_preserves_scope_exp; eauto.
+      constructor; auto.
+      constructor.
+    }
+    apply H6 in HC_e1. 2: rewrite <- plug_assoc in *; simpl; auto.
+    apply H7 in HC_e2. 2: rewrite <- plug_assoc in *; simpl; auto.
+    rewrite <- plug_assoc in HC_e2. simpl in HC_e2.
+    shelve.
+  * unfold CompatibleLetRec.
+    intros.
+    unfold CTX in *.
+    intuition auto.
+    rewrite H in H1; constructor; auto.
+    clear H5 H9 H6 H10.
+    assert (EECTX S (length vl) + Γ ⊢ plugc C (CLetRec1 f vl CHole e2) ∷ 0) as HC_e1.
+    { eapply plugc_preserves_scope_exp; eauto.
+      constructor; auto.
+      constructor.
+    }
+    assert (EECTX S Γ ⊢ plugc C (CLetRec2 f vl b1' CHole) ∷ 0) as HC_e2.
+    { eapply plugc_preserves_scope_exp; eauto.
+      constructor; auto.
+      constructor.
+    }
+    apply H7 in HC_e1. 2: rewrite <- plug_assoc in *; simpl; auto.
+    apply H8 in HC_e2. 2: rewrite <- plug_assoc in *; simpl; auto.
+    rewrite <- plug_assoc in HC_e2. simpl in HC_e2.
+    shelve.
+  * unfold CompatibleCase.
+    intros.
+    unfold CTX in *.
+    intuition auto.
+    clear H7 H12 H8 H13 H5 H14.
+    assert (EECTX Γ ⊢ plugc C (CCase1 CHole p e2 e3) ∷ 0) as HC_e1.
+    { eapply plugc_preserves_scope_exp; eauto.
+      constructor; auto.
+      constructor.
+    }
+    apply H9 in HC_e1. 2: rewrite <- plug_assoc; simpl; auto.
+    assert (EECTX pat_vars p + Γ ⊢ plugc C (CCase2 e1' p CHole e3) ∷ 0) as HC_e2.
+    { eapply plugc_preserves_scope_exp; eauto.
+      constructor; auto.
+      constructor.
+    }
+    apply H10 in HC_e2. 2: { rewrite <- plug_assoc in *; simpl in *; auto. }
+    assert (EECTX Γ ⊢ plugc C (CCase3 e1' p e2' CHole) ∷ 0) as HC_e3.
+    { eapply plugc_preserves_scope_exp; eauto.
+      constructor; auto.
+      constructor.
+    }
+    apply H11 in HC_e3. 2: { rewrite <- plug_assoc in *; simpl in *; auto. }
+    rewrite <- plug_assoc in HC_e3. simpl in HC_e3. auto.
+  * unfold CompatibleCons.
+    intros.
+    unfold CTX in *.
+    intuition auto.
+    clear H4 H8 H5 H9.
+    assert (EECTX Γ ⊢ plugc C (CCons1 e1 CHole) ∷ 0) as HC_e1.
+    { eapply plugc_preserves_scope_exp; eauto.
+      constructor; auto.
+      constructor.
+    }
+    apply H7 in HC_e1. 2: rewrite <- plug_assoc; simpl; auto.
+    assert (EECTX Γ ⊢ plugc C (CCons2 CHole e2') ∷ 0) as HC_e2.
+    { eapply plugc_preserves_scope_exp; eauto.
+      constructor; auto.
+      constructor.
+    }
+    apply H6 in HC_e2. 2: rewrite <- plug_assoc in *; simpl; auto.
+    rewrite <- plug_assoc in HC_e2. simpl in HC_e2; auto.
+  * unfold CompatibleBIF.
+    intros.
+    unfold CTX in *.
+    intuition auto.
+    1-2: rewrite indexed_to_forall in H, H0; constructor; auto.
+    clear H3 H7.
+    assert (EECTX Γ ⊢ plugc C (CBIFFun CHole vals1) ∷ 0) as HC_e1.
+    { eapply plugc_preserves_scope_exp; eauto.
+      constructor; auto.
+      constructor.
+    }
+    apply H6 in HC_e1. 2: rewrite <- plug_assoc in *; simpl; auto.
+    apply biforall_length in H4 as LL. rewrite <- plug_assoc in HC_e1.
+    destruct vals1; intros.
+    - inversion H4. now subst.
+    - inversion H4. subst. destruct H9, H3. inversion H. inversion H0. subst.
+      assert (EECTX Γ ⊢ plugc C (CBIFParam f2 [] CHole vals1) ∷ 0). {
+        eapply plugc_preserves_scope_exp; eauto.
+        constructor; auto.
+        constructor.
+      }
+      apply H7 in H10. 2: now rewrite <- plug_assoc.
+      replace (hd' :: tl') with ([] ++ [hd'] ++ tl') by auto.
+      eapply PreCTX_BIF_helper; eauto.
+      now rewrite plug_assoc.
+  * unfold CompatibleReceive.
+    intros.
+    unfold CTX in *.
+    split. split.
+    (** TODO: will be changed *)
+    3: { intros. destruct l, l2. 2-3: inversion H1.
+         auto.
+         destruct p, p0. inversion H1. subst. destruct H7 as [H7_1 [ [H7_21 H7_22] H7_3]].
+         pose proof (PreCTX_rec_helper l l2 C Γ e p [] H2 ltac:(constructor) H3 H9 H7_21).
+         simpl in H4. subst.
+         epose proof (P := H7_3 (plugc C (CReceive [] p0 CHole l2)) _). do 2 rewrite <- plug_assoc in P.
+         simpl in P. apply P. auto.
+        }
+    all: shelve.
+Unshelve.
+    9-10: rewrite (indexed_to_forall _ _ (PNil, ELit 0%Z)) in H;
+         rewrite (indexed_to_forall _ _ (PNil, ELit 0%Z)) in H0;
+         constructor; intros.
+    9-10: replace (ELit 0%Z) with (snd (PNil, ELit 0%Z)) by auto.
+    9-10: replace 0 with ((fst >>> pat_vars) (PNil, ELit 0%Z)) by auto.
+    9-10: do 2 rewrite map_nth.
+    9: apply H in H2. 10: apply H0 in H2. 9-10: break_match_hyp; apply H2.
+  2-3, 6-7: exact (ELit 0%Z).
+  apply alpha_eval in H4; apply alpha_eval; rewrite default_context in *;
+       simpl in *; rewrite map_const in *; rewrite <- H; auto.
 
+  apply alpha_eval. apply alpha_eval in HC_e2. rewrite default_context in *. exact HC_e2.
+
+  apply alpha_eval. apply alpha_eval in HC_e2. rewrite default_context in *.
+  simpl in *; rewrite map_const in *; rewrite <- H; auto.
+
+  eapply plugc_preserves_scope_exp. exact H2. constructor. constructor.
+  intros. inversion H5.
+  intros. rewrite (indexed_to_forall _ _ (PNil, ELit 0%Z)) in H0.
+  specialize (H0 (S i) ltac:(simpl;lia)).
+  simpl in H0.
+  replace (ELit 0%Z) with (snd (PNil, ELit 0%Z)) by auto.
+  replace 0 with ((fst >>> pat_vars) (PNil, ELit 0%Z)) by auto.
+  do 2 rewrite map_nth.
+  break_match_hyp; cbn. auto.
+Qed.
+
+Lemma CTX_IsCtxRel : IsCtxRel CTX.
+Proof.
+  unfold IsCtxRel.
+  split.
+  - apply CTX_IsPreCtxRel.
+  - intros.
+    eapply CTX_bigger; eauto.
+Qed.
+
+Global Hint Resolve CTX_IsCtxRel : core.
+Global Hint Resolve CTX_IsPreCtxRel : core.
+
+Corollary CIU_implies_CTX :
+  forall Γ e1 e2, CIU_open Γ e1 e2 -> CTX Γ e1 e2.
+Proof.
+  intros. eapply CTX_bigger. 2: exact H. apply CIU_IsPreCtxRel.
+Qed.
+
+Global Hint Resolve CIU_implies_CTX : core.
+
+Lemma exists_CTX : exists R, IsCtxRel R.
+Proof.
+  exists CTX.
+  apply CTX_IsCtxRel.
+Qed.
+
+
+
+
+Lemma CIU_beta_value : forall {Γ e2 x v},
+    EXP S Γ ⊢ e2 -> VAL Γ ⊢ v ->
+    (CIU_open Γ e2.[v/] (ELet x v e2) /\ 
+     CIU_open Γ (ELet x v e2) e2.[v/]).
+Proof.
+  unfold CIU_open.
+  intros.
+  unfold CIU.
+  intuition idtac.
+  1,5: apply -> subst_preserves_scope_exp; try eassumption;
+    apply -> subst_preserves_scope_exp; eauto.
+  1,3: simpl; constructor; [ constructor; apply -> subst_preserves_scope_val; eauto |
+                             apply -> subst_preserves_scope_exp; eauto ].
+  destruct H3. exists (S (S x0)). simpl. apply term_let.
+  pose proof (subst_preserves_scope_val v Γ). destruct H4.
+  clear H5. specialize (H4 H0 0 ξ H1). constructor; auto.
+  rewrite subst_comp, subst_extend.
+  now rewrite subst_comp, scons_substcomp, substcomp_id_l in H3.
+
+  destruct H3. simpl in H3. inversion H3; try inversion_is_value. subst.
+  pose proof (subst_preserves_scope_val v Γ). destruct H4.
+  clear H5. specialize (H4 H0 0 ξ H1).
+  inversion H9; subst.
+  rewrite subst_comp, subst_extend in H12.
+  rewrite subst_comp, scons_substcomp, substcomp_id_l. eexists. exact H12.
+
+  all: rewrite <- H5 in H4; inversion H4.
+Qed.
+
+Lemma CTX_closed_under_substitution : forall {Γ e1 e2 v R},
+    IsCtxRel R ->
+    VAL Γ ⊢ v ->
+    R (S Γ) e1 e2 ->
+    R Γ e1.[v/] e2.[v/].
+Proof.
+  intros Γ e1 e2 v R HCtx Hscope_v HCtx_e1e2.
+  destruct HCtx as [HCtx Hbiggest].
+  destruct HCtx as [Rscope [Radequate [Rrefl [Rtrans [RFun [RApp [RLet [RLetRec [RPlus RIf]]]]]]]]].
+  destruct (Rscope _ _ _ HCtx_e1e2) as [Hscope_e1 Hscope_e2].
+  epose proof (@CIU_beta_value Γ e1 "X"%string v Hscope_e1 _).
+  epose proof (@CIU_beta_value Γ e2 "X"%string v Hscope_e2 _).
+  destruct H as [? _].
+  destruct H0 as [_ ?].
+  apply CIU_iff_Erel in H.
+  apply CIU_iff_Erel in H0.
+  apply Hbiggest in H; auto using Erel_IsPreCtxRel.
+  apply Hbiggest in H0; auto using Erel_IsPreCtxRel.
+  eapply Rtrans in H.
+  eapply H.
+  eapply Rtrans; revgoals.
+  eapply H0.
+  apply RLet.
+  1-2: constructor; auto.
+  1-2: auto.
+  apply Rrefl. now constructor.
+  auto.
+Unshelve.
+  1-2: auto.
+Qed.
+
+Theorem CIU_IsCtxRel : IsCtxRel CIU_open.
+Proof.
+  destruct exists_CTX as [R' HR'].
+  eapply bigger_implies_IsCtxRel. 2: eauto using CIU_IsPreCtxRel. apply CTX_IsCtxRel.
+  induction Γ; revgoals.
+  - unfold CIU_open.
+    intros.
+    pose proof (H0 0 ltac:(lia)). break_match_hyp. 2: inversion H1.
+    replace e1.[ξ] with e1.[e/].[(fun n => n + 1) >>> ξ]; revgoals.
+    {
+      rewrite subst_comp. rewrite scons_substcomp_core.
+      rewrite (vclosed_ignores_sub e); auto.
+      rewrite <- substcomp_scons, idsubst_up, substcomp_id_l.
+      now rewrite subst_ren_scons.
+    }
+    replace e2.[ξ] with e2.[e/].[(fun n => n + 1) >>> ξ]; revgoals.
+    {
+      rewrite subst_comp. rewrite scons_substcomp_core.
+      rewrite (vclosed_ignores_sub e); auto.
+      rewrite <- substcomp_scons, idsubst_up, substcomp_id_l.
+      now rewrite subst_ren_scons.
+    }
+    apply IHΓ.
+    apply CTX_closed_under_substitution; auto; revgoals.
+    + specialize (H0 0 ltac:(lia)).
+      simpl. replace e with (e.[idsubst]) by auto.
+      apply -> subst_preserves_scope_val; eauto. intro. intros. inversion H2.
+    + unfold subscoped.
+      intros. apply H0. lia.
+  - unfold CIU_open.
+    intros.
+    unfold CIU.
+    intuition idtac.
+    + apply -> subst_preserves_scope_exp; eauto. destruct HR'.
+      eapply H1 with (e1:=e1) (e2:=e2). apply H2 in H; auto.
+    + apply -> subst_preserves_scope_exp; eauto 3. destruct HR'.
+      eapply H1 with (e1:=e1) (e2:=e2); eauto 3.
+    + replace e1.[ξ] with e1 in H2; revgoals.
+      { replace ξ with (upn 0 ξ) by auto.
+        rewrite escoped_ignores_sub; auto. destruct HR'.
+        eapply H3 with (e1:=e1) (e2:=e2); eauto.
+      }
+      replace e2.[ξ] with e2; revgoals.
+      { replace ξ with (upn 0 ξ) by auto.
+        rewrite escoped_ignores_sub; auto. destruct HR'.
+        eapply H3 with (e1:=e1) (e2:=e2); eauto.
+      }
+      clear H0.
+      generalize dependent e2. generalize dependent e1. generalize dependent F.
+      induction F; intros.
+      * destruct HR'. destruct H, H. apply (H4 CHole); auto. constructor.
+      * inversion H1. subst.
+        assert (EXPCLOSED e1) as EC1 by apply H.
+        assert (EXPCLOSED e2) as EC2 by apply H.
+        apply put_back in H2; auto. destruct H2. apply put_back_rev; auto.
+        eapply IHF; auto. exists x. exact H0.
+        destruct HR'. inversion H. clear H6.
+        destruct a; inversion H4; subst.
+        -- simpl. apply CTX_IsPreCtxRel; auto. apply forall_biforall_refl.
+           apply Forall_forall. intros. apply CTX_refl. rewrite Forall_forall in H8.
+           now apply H8.
+        -- simpl. apply CTX_IsPreCtxRel; auto.
+           ++ apply Forall_app. split; auto. eapply Forall_impl. 2: exact H12.
+              intros. now constructor.
+           ++ apply Forall_app. split; auto. eapply Forall_impl. 2: exact H12.
+              intros. now constructor.
+           ++ apply CTX_refl. now constructor.
+           ++ apply biforall_app. 2: constructor; auto.
+              all: apply forall_biforall_refl; apply Forall_forall; 
+                   intros; apply CTX_refl; rewrite Forall_forall in H11, H12.
+              constructor. now apply H12.
+              now apply H11.
+        -- simpl. apply CTX_IsPreCtxRel; auto. now apply CTX_refl.
+        -- simpl. apply CTX_IsPreCtxRel; auto.
+           1-2: now rewrite Nat.add_0_r. 1-2: apply CTX_refl; auto; now rewrite Nat.add_0_r.
+        -- simpl. apply CTX_IsPreCtxRel; auto. now apply CTX_refl.
+        -- simpl. apply CTX_IsPreCtxRel; auto.
+           apply CTX_refl.
+           all: apply scoped_val; auto.
+        -- simpl. apply CTX_IsPreCtxRel; auto. apply forall_biforall_refl.
+           apply Forall_forall. intros. apply CTX_refl. rewrite Forall_forall in H8.
+           now apply H8.
+        -- simpl. apply CTX_IsPreCtxRel; auto.
+           ++ apply Forall_app. split; auto. eapply Forall_impl. 2: exact H12.
+              intros. now constructor.
+           ++ apply Forall_app. split; auto. eapply Forall_impl. 2: exact H12.
+              intros. now constructor.
+           ++ apply CTX_refl. now constructor.
+           ++ apply biforall_app. 2: constructor; auto.
+              all: apply forall_biforall_refl; apply Forall_forall; 
+                   intros; apply CTX_refl; rewrite Forall_forall in H11, H12.
+              constructor. now apply H12.
+              now apply H11.
+Qed.
+
+Theorem Erel_IsCtxRel : IsCtxRel Erel_open.
+Proof.
+  unfold IsCtxRel.
+  split.
+  apply Erel_IsPreCtxRel.
+  intros.
+  apply CIU_iff_Erel.
+  pose proof CIU_IsCtxRel.
+  unfold IsCtxRel in H1.
+  destruct H1.
+  eapply H2; eauto.
+Qed.
+
+Corollary CTX_implies_CIU :
+  forall e1 e2 Γ, CTX Γ e1 e2 -> CIU_open Γ e1 e2.
+Proof.
+  intros. eapply CIU_IsCtxRel. 2: exact H. auto.
+Qed.
+
+Global Hint Resolve CTX_implies_CIU : core.
+
+Corollary CIU_iff_CTX :
+  forall e1 e2 Γ, CTX Γ e1 e2 <-> CIU_open Γ e1 e2.
+Proof.
+  intros. split; auto.
+Qed.
+
+Corollary Erel_iff_CTX :
+  forall e1 e2 Γ, CTX Γ e1 e2 <-> Erel_open Γ e1 e2.
+Proof.
+  intros. split; intros.
+  * apply CIU_iff_Erel. auto.
+  * apply CIU_iff_Erel in H. auto.
+Qed.
+
+Corollary CTX_eval : forall e1 v,
+  EXPCLOSED e1 ->
+  ⟨ [], e1 ⟩ -->* v -> CTX 0 e1 v /\ CTX 0 v e1.
+Proof.
+  intros. split; apply CIU_iff_CTX; intro; intros.
+  rewrite eclosed_ignores_sub, vclosed_ignores_sub.
+  4: rewrite vclosed_ignores_sub, eclosed_ignores_sub.
+  1, 4: pose proof (CIU_eval _ _ H H0). all: auto. 1-2: apply H2.
+  all: apply step_any_closedness in H0; auto; constructor.
+Qed.
 
